theories/allocator/allocator_free_spec.v
@@ -1,0 +1,882 @@
+From iris.proofmode Require Import proofmode.
+From griotte Require Import rules proofmode memory_region.
+From griotte.allocator Require Import allocator_preamble
+  allocator_macros_spec.
+
+(** Address of an assembled block relative to the entry point. *)
+Definition allocator_free_block_addr {MP : MachineParameters}
+  (pc_a : Addr) (n : nat) : Addr :=
+  (pc_a ^+ length (concat (take n assembled_allocator_free)))%a.
+
+Section AllocatorFreeBlocks.
+  Context {Σ : gFunctors} {ceriseg : ceriseG Σ} {allocatorg : allocatorG Σ}
+    {MP : MachineParameters} {layout : allocatorLayout}.
+
+  Lemma allocator_free_success_block_spec
+    (E : coPset) (pc_b pc_e pc_a : Addr) (wreq wstatus : Word)
+    (φ : language.val griotte_lang → iPropI Σ) :
+
+    let start := allocator_free_block_addr pc_a 5 in
+    let code := allocator_free_instrs_n 5 in
+    ContiguousRegion pc_a (length allocator_free_instrs) ->
+    SubBounds pc_b pc_e pc_a (pc_a ^+ length allocator_free_instrs)%a ->
+    disjoint_from_shadow pc_b pc_e ->
+
+    ▷ PC ↦ᵣ WCap true RX Global pc_b pc_e start
+    ∗ ▷ ca0 ↦ᵣ wreq
+    ∗ ▷ ca1 ↦ᵣ wstatus
+    ∗ ▷ codefrag start code
+    ∗ ▷ (PC ↦ᵣ WCap true RX Global pc_b pc_e
+           (allocator_free_block_addr pc_a 7)
+         ∗ ca0 ↦ᵣ WInt 0
+         ∗ ca1 ↦ᵣ WInt ALLOC_OK
+         ∗ codefrag start code
+         -∗ WP Seq (Instr Executable) @ E {{ φ }})
+    ⊢ WP Seq (Instr Executable) @ E {{ φ }}.
+  Proof.
+    intros start code Hcont Hpc Hshadow; subst start code.
+    iIntros "(>HPC & >Hca0 & >Hca1 & >Hcode & Hφ)".
+    codefrag_facts "Hcode".
+    (* Mov ca0 0. *)
+    iInstr "Hcode".
+    assert (Hstep : (pc_a ^+ 37)%a =
+      ((allocator_free_block_addr pc_a 5) ^+ 1)%a).
+    { unfold allocator_free_block_addr. solve_addr. }
+    iEval (rewrite Hstep) in "HPC".
+    (* Mov ca1 ALLOC_OK. *)
+    iInstr "Hcode".
+    (* Jmp .free_return. *)
+    iInstr "Hcode".
+    assert (Hret : (allocator_free_block_addr pc_a 5 ^+ 5)%a =
+      allocator_free_block_addr pc_a 7).
+    { unfold allocator_free_block_addr. solve_addr. }
+    iEval (rewrite Hret) in "HPC".
+    iApply "Hφ". iFrame.
+  Qed.
+
+  Lemma allocator_free_prepare_valid_spec
+    (E : coPset)
+    (pc_b pc_e pc_a next : Addr)
+    (wreq w0 w1 w2 w3 : Word)
+    (φ : language.val griotte_lang → iPropI Σ) :
+
+    let code := allocator_free_instrs_n 0 ++ allocator_free_instrs_n 1 in
+    allocatorLayoutWf ->
+    ↑Nallocator ⊆ E ->
+    ContiguousRegion pc_a (length allocator_free_instrs) ->
+    SubBounds pc_b pc_e pc_a (pc_a ^+ length allocator_free_instrs)%a ->
+    disjoint_from_shadow pc_b pc_e ->
+    allocator_free_valid next wreq ->
+
+    allocator_ctx
+    ∗ allocator_service_data next
+    ∗ ▷ PC ↦ᵣ WCap true RX Global pc_b pc_e pc_a
+    ∗ ▷ cgp ↦ᵣ WCap true RW Global
+        allocator_cgp_b allocator_cgp_e allocator_cgp_b
+    ∗ ▷ ca0 ↦ᵣ wreq
+    ∗ ▷ ct0 ↦ᵣ w0
+    ∗ ▷ ct1 ↦ᵣ w1
+    ∗ ▷ ct2 ↦ᵣ w2
+    ∗ ▷ ct3 ↦ᵣ w3
+    ∗ ▷ codefrag pc_a code
+    ∗ ▷ (allocator_service_data next
+         ∗ cgp ↦ᵣ WCap true RW Global
+             allocator_cgp_b allocator_cgp_e allocator_cgp_b
+         ∗ ca0 ↦ᵣ wreq
+         ∗ codefrag pc_a code
+         ∗ (∃ (p : Perm) (g : Locality) (b e a : Addr),
+             ⌜wreq = WCap true p g b e a
+               ∧ (heap_b < b /\ b < e /\ e <= next)%a⌝
+             ∗ PC ↦ᵣ WCap true RX Global pc_b pc_e
+                 (allocator_free_block_addr pc_a 2)
+             ∗ ct0 ↦ᵣ WCap true RW Global heap_b heap_e next
+             ∗ ct1 ↦ᵣ WInt b
+             ∗ ct2 ↦ᵣ WInt e
+             ∗ ct3 ↦ᵣ WInt 0)
+         -∗ WP Seq (Instr Executable) @ E {{ φ }})
+    ⊢ WP Seq (Instr Executable) @ E {{ φ }}.
+  Proof.
+    intros code Hlayout HE Hcont Hpc Hdisjoint (p & g & b & e & a & -> & Hbounds); subst code.
+    iIntros "(#Hctx & Hdata & >HPC & >Hcgp & >Hca0 & >Hct0 & >Hct1 & >Hct2 & >Hct3 & >Hcode & Hφ)".
+    iDestruct "Hdata" as "(%Hnext & Hslot & Hroot & Hfree)".
+    codefrag_facts "Hcode".
+    (* GetWType ct3 ca0. *)
+    iInstr "Hcode".
+    (* Sub ct3 ct3 (encodeWordType wt_cap). *)
+    iInstr "Hcode".
+    rewrite (encodeWordType_correct_cap true p g b e a true (O LG LM) Global 0%a 0%a 0%a) /wt_cap Z.sub_diag.
+    (* Jnz .free_invalid ct3 falls through for a capability. *)
+    iInstr "Hcode".
+    (* GetTag ct3 ca0. *)
+    iInstr "Hcode".
+    (* Sub ct3 ct3 1. *)
+    iInstr "Hcode".
+    rewrite /Z.b2z Z.sub_diag.
+    (* Jnz .free_invalid ct3 falls through for a tagged capability. *)
+    iInstr "Hcode".
+    (* Load ct0 cgp reads the stored bump capability with its clear root shadow bit. *)
+    iInstr_lookup "Hcode" as "Hi" "Hcode".
+    wp_instr.
+    iDestruct (allocator_free_cell_shadow_access heap_b with "Hctx") as "#Haccess".
+    {
+      apply elem_of_heap_addresses.
+      apply withinBounds_true_iff.
+      pose proof heap_valid.
+      solve_addr.
+    }
+    iApply (wp_atomic _ _ (E ∖ ↑Nallocator)).
+    iMod ("Haccess" $! E HE with "Hroot") as (bit Hbit) "[Hs Hclose]".
+    subst bit.
+    iModIntro.
+    iApply (wp_load_success_heap with "[$HPC $Hi $Hct0 $Hcgp $Hslot $Hs]"); try solve_pure.
+    {
+      eapply (disjoint_from_shadow_not_in allocator_cgp_b allocator_cgp_e allocator_cgp_b).
+      { pose proof (@allocator_regions_disjoint MP layout Hlayout) as Hregions.
+        unfold disjoint_from_shadow.
+        rewrite !disjoint_list_cons in Hregions.
+        cbn [union_list] in Hregions.
+        set_solver. }
+      { apply withinBounds_true_iff.
+        pose proof (@allocator_size_data MP layout Hlayout) as Hsize.
+        cbn in Hsize.
+        solve_addr. }
+    }
+    {
+      unfold is_heap_address.
+      apply withinBounds_true_iff.
+      pose proof heap_valid.
+      solve_addr.
+    }
+    {
+      split; first done.
+      apply withinBounds_true_iff.
+      pose proof (@allocator_size_data MP layout Hlayout) as Hsize.
+      cbn in Hsize.
+      solve_addr.
+    }
+    iIntros "!> (HPC & Hct0 & Hi & Hcgp & Hslot & Hs)".
+    iMod ("Hclose" with "Hs") as "Hroot".
+    iModIntro.
+    wp_pure.
+    iSpecialize ("Hcode" with "Hi").
+    iEval (simpl) in "Hct0".
+    (* GetB ct1 ca0. *)
+    iInstr "Hcode".
+    (* GetE ct2 ca0. *)
+    iInstr "Hcode".
+    (* GetB ct3 ct0. *)
+    iInstr "Hcode".
+    (* Lt ct3 ct3 ct1 tests heap_b < b. *)
+    iInstr "Hcode".
+    replace (heap_b <? b)%Z with true by (symmetry; apply Z.ltb_lt; solve_addr).
+    (* Jnz .free_base_ok ct3 skips the invalid jump. *)
+    iInstr "Hcode".
+    (* Lt ct3 ct1 ct2 tests b < e. *)
+    iInstr "Hcode".
+    replace (b <? e)%Z with true by (symmetry; apply Z.ltb_lt; solve_addr).
+    (* Jnz .free_nonempty ct3 skips the invalid jump. *)
+    iInstr "Hcode".
+    (* GetA ct3 ct0 reads the bump cursor. *)
+    iInstr "Hcode".
+    (* Lt ct3 ct3 ct2 tests next < e. *)
+    iInstr "Hcode".
+    replace (next <? e)%Z with false by (symmetry; apply Z.ltb_ge; solve_addr).
+    (* Jnz .free_invalid ct3 falls through for e <= next. *)
+    iInstr "Hcode".
+    iApply "Hφ".
+    iSplitL "Hslot Hroot Hfree".
+    { iFrame. done. }
+    iFrame "Hcgp Hca0 Hcode".
+    iExists p, g, b, e, a.
+    iSplit.
+    { iPureIntro. split; first done. exact Hbounds. }
+    iFrame.
+  Qed.
+
+  Lemma allocator_free_prepare_invalid_spec
+    (E : coPset)
+    (pc_b pc_e pc_a next : Addr)
+    (wreq w0 w1 w2 w3 : Word)
+    (φ : language.val griotte_lang → iPropI Σ) :
+
+    let code := allocator_free_instrs_n 0 ++ allocator_free_instrs_n 1 in
+    allocatorLayoutWf ->
+    ↑Nallocator ⊆ E ->
+    ContiguousRegion pc_a (length allocator_free_instrs) ->
+    SubBounds pc_b pc_e pc_a (pc_a ^+ length allocator_free_instrs)%a ->
+    disjoint_from_shadow pc_b pc_e ->
+    ¬ allocator_free_valid next wreq ->
+
+    allocator_ctx
+    ∗ allocator_service_data next
+    ∗ ▷ PC ↦ᵣ WCap true RX Global pc_b pc_e pc_a
+    ∗ ▷ cgp ↦ᵣ WCap true RW Global
+        allocator_cgp_b allocator_cgp_e allocator_cgp_b
+    ∗ ▷ ca0 ↦ᵣ wreq
+    ∗ ▷ ct0 ↦ᵣ w0
+    ∗ ▷ ct1 ↦ᵣ w1
+    ∗ ▷ ct2 ↦ᵣ w2
+    ∗ ▷ ct3 ↦ᵣ w3
+    ∗ ▷ codefrag pc_a code
+    ∗ ▷ (allocator_service_data next
+         ∗ cgp ↦ᵣ WCap true RW Global
+             allocator_cgp_b allocator_cgp_e allocator_cgp_b
+         ∗ ca0 ↦ᵣ wreq
+         ∗ codefrag pc_a code
+         ∗ PC ↦ᵣ WCap true RX Global pc_b pc_e
+             (allocator_free_block_addr pc_a 6)
+         ∗ ct0 ↦ᵣ -
+         ∗ ct1 ↦ᵣ -
+         ∗ ct2 ↦ᵣ -
+         ∗ ct3 ↦ᵣ -
+         -∗ WP Seq (Instr Executable) @ E {{ φ }})
+    ⊢ WP Seq (Instr Executable) @ E {{ φ }}.
+  Proof.
+    intros code Hlayout HE Hcont Hpc Hdisjoint Hrequest; subst code.
+    iIntros "(#Hctx & Hdata & >HPC & >Hcgp & >Hca0 & >Hct0 & >Hct1 & >Hct2 & >Hct3 & >Hcode & Hφ)".
+    iDestruct "Hdata" as "(%Hnext & Hslot & Hroot & Hfree)".
+    codefrag_facts "Hcode".
+    (* GetWType ct3 ca0. *)
+    iInstr "Hcode".
+    (* Sub ct3 ct3 (encodeWordType wt_cap). *)
+    iInstr "Hcode".
+    destruct (is_cap wreq) eqn:Hreq_cap.
+    + destruct wreq; cbn in Hreq_cap; try done.
+      destruct sb; cbn in Hreq_cap; try done.
+      rewrite (encodeWordType_correct_cap tag p g b e a true (O LG LM) Global 0%a 0%a 0%a) /wt_cap Z.sub_diag.
+      (* Jnz .free_invalid ct3 falls through for a capability. *)
+      iInstr "Hcode".
+      (* GetTag ct3 ca0. *)
+      iInstr "Hcode".
+      (* Sub ct3 ct3 1. *)
+      iInstr "Hcode".
+      destruct tag.
+      * rewrite /Z.b2z Z.sub_diag.
+        (* Jnz .free_invalid ct3 falls through for a tagged capability. *)
+        iInstr "Hcode".
+        (* Load ct0 cgp reads the stored bump capability with its clear root shadow bit. *)
+        iInstr_lookup "Hcode" as "Hi" "Hcode".
+        wp_instr.
+        iDestruct (allocator_free_cell_shadow_access heap_b with "Hctx") as "#Haccess".
+        {
+          apply elem_of_heap_addresses.
+          apply withinBounds_true_iff.
+          pose proof heap_valid.
+          solve_addr.
+        }
+        iApply (wp_atomic _ _ (E ∖ ↑Nallocator)).
+        iMod ("Haccess" $! E HE with "Hroot") as (bit Hbit) "[Hs Hclose]".
+        subst bit.
+        iModIntro.
+        iApply (wp_load_success_heap with "[$HPC $Hi $Hct0 $Hcgp $Hslot $Hs]"); try solve_pure.
+        {
+          eapply (disjoint_from_shadow_not_in allocator_cgp_b allocator_cgp_e allocator_cgp_b).
+          { pose proof (@allocator_regions_disjoint MP layout Hlayout) as Hregions.
+            unfold disjoint_from_shadow.
+            rewrite !disjoint_list_cons in Hregions.
+            cbn [union_list] in Hregions.
+            set_solver. }
+          { apply withinBounds_true_iff.
+            pose proof (@allocator_size_data MP layout Hlayout) as Hsize.
+            cbn in Hsize.
+            solve_addr. }
+        }
+        {
+          unfold is_heap_address.
+          apply withinBounds_true_iff.
+          pose proof heap_valid.
+          solve_addr.
+        }
+        {
+          split; first done.
+          apply withinBounds_true_iff.
+          pose proof (@allocator_size_data MP layout Hlayout) as Hsize.
+          cbn in Hsize.
+          solve_addr.
+        }
+        iIntros "!> (HPC & Hct0 & Hi & Hcgp & Hslot & Hs)".
+        iMod ("Hclose" with "Hs") as "Hroot".
+        iModIntro.
+        wp_pure.
+        iSpecialize ("Hcode" with "Hi").
+        iEval (simpl) in "Hct0".
+        (* GetB ct1 ca0. *)
+        iInstr "Hcode".
+        (* GetE ct2 ca0. *)
+        iInstr "Hcode".
+        (* GetB ct3 ct0. *)
+        iInstr "Hcode".
+        (* Lt ct3 ct3 ct1 tests heap_b < b. *)
+        iInstr "Hcode".
+        destruct (decide (heap_b < b)%a) as [Hbase|Hbase].
+        ** replace (heap_b <? b)%Z with true by (symmetry; apply Z.ltb_lt; solve_addr).
+          (* Jnz .free_base_ok ct3 skips the invalid jump. *)
+          iInstr "Hcode".
+          (* Lt ct3 ct1 ct2 tests b < e. *)
+          iInstr "Hcode".
+          destruct (decide (b < e)%a) as [Hnonempty|Hempty].
+          {
+            replace (b <? e)%Z with true by (symmetry; apply Z.ltb_lt; solve_addr).
+            (* Jnz .free_nonempty ct3 skips the invalid jump. *)
+            iInstr "Hcode".
+            (* GetA ct3 ct0 reads the bump cursor. *)
+            iInstr "Hcode".
+            (* Lt ct3 ct3 ct2 tests next < e. *)
+            iInstr "Hcode".
+            destruct (decide (next < e)%a) as [Hpast|Hwithin].
+            {
+              replace (next <? e)%Z with true by (symmetry; apply Z.ltb_lt; solve_addr).
+              (* Jnz .free_invalid ct3 rejects e > next. *)
+              iInstr "Hcode".
+              iApply "Hφ". iFrame. done.
+            }
+            { exfalso. apply Hrequest.
+              exists p, g, b, e, a. split; first reflexivity. solve_addr. }
+          }
+          replace (b <? e)%Z with false by (symmetry; apply Z.ltb_ge; solve_addr).
+          (* Jnz .free_nonempty ct3 falls through for an empty interval. *)
+          iInstr "Hcode".
+          (* Jmp .free_invalid rejects an empty interval. *)
+          iInstr "Hcode".
+          iApply "Hφ". iFrame. done.
+        ** replace (heap_b <? b)%Z with false by (symmetry; apply Z.ltb_ge; solve_addr).
+          (* Jnz .free_base_ok ct3 falls through for an invalid base. *)
+          iInstr "Hcode".
+          (* Jmp .free_invalid rejects a base outside the heap prefix. *)
+          iInstr "Hcode".
+          iApply "Hφ". iFrame. done.
+      * cbn.
+        (* Jnz .free_invalid ct3 rejects an untagged capability. *)
+        iInstr "Hcode".
+        iApply "Hφ". iFrame. done.
+    + assert (Hnoncap : WInt (encodeWordType wreq - encodeWordType wt_cap) ≠ WInt 0).
+      {
+        pose proof (encodeWordType_correct wreq wt_cap) as Hencode.
+        intro Hzero.
+        injection Hzero as Hzero.
+        assert (Heq : encodeWordType wreq = encodeWordType wt_cap) by lia.
+        destruct wreq; cbn in Hreq_cap, Hencode; try discriminate.
+        all: try (destruct sb; cbn in Hreq_cap, Hencode; try discriminate); contradiction.
+      }
+      (* Jnz .free_invalid ct3 rejects a non-capability word. *)
+      iInstr "Hcode".
+      iApply "Hφ". iFrame. done.
+  Qed.
+End AllocatorFreeBlocks.
+
+Section AllocatorFreeProof.
+  Context
+    {Σ : gFunctors}
+    {ceriseg : ceriseG Σ}
+    {allocatorg : allocatorG Σ}
+    {MP : MachineParameters}
+    {layout : allocatorLayout}
+    {layout_wf : allocatorLayoutWf}
+  .
+
+  (** Since the service invariant hides the bump cursor, this class of requests
+      is invalid for every possible cursor. It includes [WInt 0]. *)
+  Definition allocator_free_always_invalid (wreq : Word) : Prop :=
+    ∀ next : Addr,
+      (heap_b < next /\ next <= heap_e)%a →
+      ¬ allocator_free_valid next wreq.
+
+  Lemma allocator_memory_not_free_cell E a w :
+    ↑Nallocator ⊆ E -> a ∈ heap_addresses ->
+    allocator_ctx -∗ a ↦ₐ w -∗ free_cell_token a ={E}=∗ False.
+  Proof.
+    iIntros (HE Ha) "#Hctx Hmem Hfree".
+    iInv Nallocator as ">Hbody" "Hclose".
+    iDestruct (allocator_inv_lookup a with "Hbody") as (s) "[Hentry Hput]"; first done.
+    iDestruct (allocator_entry_memory_live with "Hentry Hmem") as %Hlive.
+    iDestruct (allocator_entry_free_token with "Hentry Hfree") as %Hfree.
+    exfalso. congruence.
+  Qed.
+
+  Lemma allocator_range_free_contradiction E b e next a ws :
+    ↑Nallocator ⊆ E ->
+    a ∈ heap_addresses ->
+    a ∈ finz.seq_between b e ->
+    a ∈ finz.seq_between next heap_e ->
+    length ws = length (finz.seq_between b e) ->
+    allocator_ctx -∗ [[b,e]] ↦ₐ [[ws]] -∗ free_cells next heap_e ={E}=∗ False.
+  Proof.
+    iIntros (HE Ha Hmem_in Hfree_in Hlen) "#Hctx Hmem Hfree".
+    destruct (list_elem_of_lookup_1 _ _ Hmem_in) as [i Hi].
+    assert (i < length ws) as Hlt by (rewrite Hlen; eapply lookup_lt_Some; eauto).
+    destruct (lookup_lt_is_Some_2 ws i Hlt) as [w Hw].
+    iDestruct (big_sepL2_lookup_acc with "Hmem") as "[Hcell Hmemclose]"; eauto.
+    iDestruct (big_sepL_elem_of with "Hfree") as "Htoken"; eauto.
+    iMod (allocator_memory_not_free_cell E a w HE Ha with "Hctx Hcell Htoken") as %[].
+  Qed.
+
+  Lemma allocator_owned_range_below_cursor E b e next ws :
+    ↑Nallocator ⊆ E ->
+    (heap_b < b /\ b < e /\ e <= heap_e)%a ->
+    (heap_b < next /\ next <= heap_e)%a ->
+    length ws = length (finz.seq_between b e) ->
+    allocator_ctx -∗ [[b,e]] ↦ₐ [[ws]] -∗ free_cells next heap_e
+      ={E}=∗ ⌜(e <= next)%a⌝ ∗ [[b,e]] ↦ₐ [[ws]] ∗ free_cells next heap_e.
+  Proof.
+    iIntros (HE Hb Hnext Hlen) "#Hctx Hmem Hfree".
+    destruct (decide (e <= next)%a) as [Hbound|Hbad].
+    { iModIntro. iFrame. iPureIntro. exact Hbound. }
+    set (a := if decide (b < next)%a then next else b).
+    assert (Ha_heap : a ∈ heap_addresses).
+    { rewrite /heap_addresses elem_of_list_to_set elem_of_finz_seq_between.
+      unfold a. destruct (decide (b < next)%a); solve_addr. }
+    assert (Ha_mem : a ∈ finz.seq_between b e).
+    { rewrite elem_of_finz_seq_between.
+      unfold a. destruct (decide (b < next)%a); solve_addr. }
+    assert (Ha_free : a ∈ finz.seq_between next heap_e).
+    { rewrite elem_of_finz_seq_between.
+      unfold a. destruct (decide (b < next)%a); solve_addr. }
+    iMod (allocator_range_free_contradiction E b e next a ws HE Ha_heap Ha_mem Ha_free Hlen with "Hctx Hmem Hfree") as %[].
+  Qed.
+
+  (** A call with an invalid request leaves client memory untouched and returns
+      [ALLOC_INVALID]. Other registers and resources can be framed. *)
+  Lemma allocator_free_invalid_correct
+    (E : coPset) (wreq wret : Word)
+    (φ : language.val griotte_lang → iPropI Σ) :
+
+    ⊢ (⌜↑Nallocator ⊆ E⌝ -∗
+       ⌜↑Nallocator_service ⊆ E⌝ -∗
+       ⌜allocator_free_always_invalid wreq⌝ -∗
+
+       allocator_ctx ∗
+       allocator_service_ctx ∗
+       na_own cerise_nais E ∗
+
+       (* Initial register file. *)
+       PC ↦ᵣ WCap true RX Global allocator_pcc_b allocator_pcc_e
+         allocator_free_pcc_addr ∗
+       cgp ↦ᵣ WCap true RW Global
+         allocator_cgp_b allocator_cgp_e allocator_cgp_b ∗
+       cra ↦ᵣ wret ∗
+       ca0 ↦ᵣ wreq ∗
+       ca1 ↦ᵣ - ∗
+       ca2 ↦ᵣ - ∗
+       ct0 ↦ᵣ - ∗
+       ct1 ↦ᵣ - ∗
+       ct2 ↦ᵣ - ∗
+       ct3 ↦ᵣ - ∗
+       ct4 ↦ᵣ - ∗
+       ctp ↦ᵣ - ∗
+       cnull ↦ᵣ - ∗
+
+       ▷ (na_own cerise_nais E ∗
+          PC ↦ᵣ updatePcPerm wret ∗
+          cgp ↦ᵣ WCap true RW Global
+            allocator_cgp_b allocator_cgp_e allocator_cgp_b ∗
+          cra ↦ᵣ wret ∗
+          ca0 ↦ᵣ WInt 0 ∗
+          ca1 ↦ᵣ WInt ALLOC_INVALID ∗
+          ca2 ↦ᵣ - ∗
+          ct0 ↦ᵣ - ∗
+          ct1 ↦ᵣ - ∗
+          ct2 ↦ᵣ - ∗
+          ct3 ↦ᵣ - ∗
+          ct4 ↦ᵣ - ∗
+          ctp ↦ᵣ - ∗
+          cnull ↦ᵣ WInt 0
+
+          -∗ WP Seq (Instr Executable) @ E {{ φ }})
+       -∗ WP Seq (Instr Executable) @ E {{ φ }})%I.
+  Proof.
+    iIntros "%HEheap %HEservice %Hinvalid".
+    iIntros "(#Hctx & #Hservice & Hna & HPC & Hcgp & Hcra & Hca0 & Hca1 & Hca2 & Hct0 & Hct1 & Hct2 & Hct3 & Hct4 & Hctp & Hcnull & Hpost)".
+    (* Open the service invariant and recover the allocator code and state. *)
+    iMod (na_inv_acc with "Hservice Hna") as "(Hinv & Hna & Hclose)"; try exact HEservice.
+    iDestruct "Hinv" as ">[Hstatic Hdata]".
+    iDestruct "Hstatic" as "[Himports Hcode]".
+    iDestruct "Hdata" as (next) "Hdata".
+    iEval (rewrite /allocator_code) in "Hcode".
+    focus_block_nochangePC 1 "Hcode" as a_free Ha_free "Hfreecode" "Hcode_cont".
+    assert (Ha_eq : a_free = allocator_free_pcc_addr).
+    { pose proof allocator_size_imports as Himports_size.
+      unfold allocator_free_pcc_addr, allocator_free_pcc_off in *.
+      solve_addr. }
+    subst a_free.
+
+    (* Check the capability and its bounds. *)
+    assert (Hsplit : allocator_free_instrs =
+      (allocator_free_instrs_n 0 ++ allocator_free_instrs_n 1) ++
+      concat (encodeInstrsW <$> drop 2 assembled_allocator_free)) by reflexivity.
+    iEval (rewrite Hsplit) in "Hfreecode".
+    focus_block_0 "Hfreecode" as "Hprepare_code" "Hfree_cont".
+    assert (Hpc : SubBounds allocator_pcc_b allocator_pcc_e
+      allocator_free_pcc_addr (allocator_free_pcc_addr ^+ length allocator_free_instrs)%a).
+    { pose proof allocator_size_code as Hsize_code.
+      rewrite /allocator_code length_app in Hsize_code.
+      unfold allocator_free_pcc_addr, allocator_free_pcc_off in *.
+      solve_addr. }
+    assert (Hdisjoint : disjoint_from_shadow allocator_pcc_b allocator_pcc_e).
+    { pose proof allocator_regions_disjoint as Hregions.
+      unfold disjoint_from_shadow.
+      rewrite !disjoint_list_cons in Hregions.
+      cbn [union_list] in Hregions.
+      set_solver. }
+    iDestruct "Hct0" as (w0) "Hct0".
+    iDestruct "Hct1" as (w1) "Hct1".
+    iDestruct "Hct2" as (w2) "Hct2".
+    iDestruct "Hct3" as (w3) "Hct3".
+    iDestruct "Hdata" as "(%Hnext & Hslot & Hroot & Hfree)".
+    assert (Hrequest : ¬ allocator_free_valid next wreq).
+    { apply Hinvalid. exact Hnext. }
+    iAssert (allocator_service_data next) with "[Hslot Hroot Hfree]" as "Hdata".
+    { iFrame. iPureIntro. exact Hnext. }
+    iApply (allocator_free_prepare_invalid_spec with
+      "[- $Hctx $Hdata $HPC $Hcgp $Hca0 $Hct0 $Hct1 $Hct2 $Hct3 $Hprepare_code]"); eauto.
+    iNext. iIntros
+      "(Hdata & Hcgp & Hca0 & Hprepare_code & HPC & Hct0 & Hct1 & Hct2 & Hct3)".
+    iDestruct ("Hfree_cont" with "Hprepare_code") as "Hfreecode".
+    iEval (rewrite -Hsplit) in "Hfreecode".
+    (* The validity check rejects the request; set ALLOC_INVALID. *)
+    assert (Hsplit6 : allocator_free_instrs =
+      concat (encodeInstrsW <$> take 6 assembled_allocator_free) ++
+      (allocator_free_instrs_n 6 ++ allocator_free_instrs_n 7)) by reflexivity.
+    iEval (rewrite Hsplit6) in "Hfreecode".
+    focus_block_nochangePC 1 "Hfreecode" as a_invalid Ha_invalid "Hinvalid_code" "Hfreecode_cont".
+    assert (Haddr : a_invalid = allocator_free_block_addr allocator_free_pcc_addr 6).
+    { unfold allocator_free_block_addr in *. solve_addr. }
+    subst a_invalid.
+    (* Mov ca0 0. *)
+    iInstr "Hinvalid_code".
+    iDestruct "Hca1" as (wca1) "Hca1".
+    changePCto ((allocator_free_block_addr allocator_free_pcc_addr 6) ^+ 1)%a.
+    (* Mov ca1 ALLOC_INVALID. *)
+    iInstr_lookup "Hinvalid_code" as "Hi" "Hinvalid_code".
+    wp_instr.
+    iApply (wp_move_success_z with "[$HPC $Hi $Hca1]"); try solve_pure.
+    iIntros "!> (HPC & Hi & Hca1)". wp_pure.
+    iSpecialize ("Hinvalid_code" with "Hi").
+    iDestruct ("Hfreecode_cont" with "Hinvalid_code") as "Hfreecode".
+    iEval (rewrite -Hsplit6) in "Hfreecode".
+
+    (* Return to the caller and restore the service invariant. *)
+    assert (Hsplit7 : allocator_free_instrs =
+      concat (encodeInstrsW <$> take 7 assembled_allocator_free) ++
+      allocator_free_instrs_n 7) by reflexivity.
+    iEval (rewrite Hsplit7) in "Hfreecode".
+    focus_block_nochangePC 1 "Hfreecode" as a_ret Ha_ret "Hret_code" "Hfreecode_cont".
+    assert (Haddr : a_ret = allocator_free_block_addr allocator_free_pcc_addr 7).
+    { unfold allocator_free_block_addr in *. solve_addr. }
+    subst a_ret.
+    changePCto (allocator_free_block_addr allocator_free_pcc_addr 7).
+    iDestruct "Hcnull" as (wnull) "Hcnull".
+    (* Jalr cnull cra. *)
+    iInstr "Hret_code".
+    iDestruct ("Hfreecode_cont" with "Hret_code") as "Hfreecode".
+    iEval (rewrite -Hsplit7) in "Hfreecode".
+    iDestruct ("Hcode_cont" with "Hfreecode") as "Hcode".
+    iEval (rewrite -/allocator_code) in "Hcode".
+    iMod ("Hclose" with "[Himports Hcode Hdata Hna]") as "Hna".
+    { iSplitR "Hna"; last iFrame.
+      iNext. iSplitL "Himports Hcode"; first iFrame.
+      iExists next. iFrame. }
+    iApply "Hpost". iFrame "∗".
+  Qed.
+
+  (** Ownership of every cell in the capability's bounds witnesses a live
+      range in the allocated prefix. A successful call relinquishes that memory
+      and returns one reclaim token per cell. Permissions and cursor may vary. *)
+  Lemma allocator_free_valid_correct
+    (E : coPset) (p : Perm) (g : Locality) (b e a : Addr)
+    (ws : list Word) (wret : Word)
+    (φ : language.val griotte_lang → iPropI Σ) :
+
+    ⊢ (⌜↑Nallocator ⊆ E⌝ -∗
+       ⌜↑Nallocator_service ⊆ E⌝ -∗
+       ⌜(heap_b < b /\ b < e /\ e <= heap_e)%a⌝ -∗
+       ⌜length ws = length (finz.seq_between b e)⌝ -∗
+
+       allocator_ctx ∗
+       allocator_service_ctx ∗
+       na_own cerise_nais E ∗
+       [[b, e]] ↦ₐ [[ws]] ∗
+
+       (* Initial register file. *)
+       PC ↦ᵣ WCap true RX Global allocator_pcc_b allocator_pcc_e
+         allocator_free_pcc_addr ∗
+       cgp ↦ᵣ WCap true RW Global
+         allocator_cgp_b allocator_cgp_e allocator_cgp_b ∗
+       cra ↦ᵣ wret ∗
+       ca0 ↦ᵣ WCap true p g b e a ∗
+       ca1 ↦ᵣ - ∗
+       ca2 ↦ᵣ - ∗
+       ct0 ↦ᵣ - ∗
+       ct1 ↦ᵣ - ∗
+       ct2 ↦ᵣ - ∗
+       ct3 ↦ᵣ - ∗
+       ct4 ↦ᵣ - ∗
+       ctp ↦ᵣ - ∗
+       cnull ↦ᵣ - ∗
+
+       ▷ (na_own cerise_nais E ∗
+          PC ↦ᵣ updatePcPerm wret ∗
+          cgp ↦ᵣ WCap true RW Global
+            allocator_cgp_b allocator_cgp_e allocator_cgp_b ∗
+          cra ↦ᵣ wret ∗
+          ca0 ↦ᵣ WInt 0 ∗
+          ca1 ↦ᵣ WInt ALLOC_OK ∗
+          ca2 ↦ᵣ - ∗
+          ct0 ↦ᵣ - ∗
+          ct1 ↦ᵣ - ∗
+          ct2 ↦ᵣ - ∗
+          ct3 ↦ᵣ - ∗
+          ct4 ↦ᵣ - ∗
+          ctp ↦ᵣ - ∗
+          cnull ↦ᵣ WInt 0 ∗
+          allocator_reclaimed b e
+
+          -∗ WP Seq (Instr Executable) @ E {{ φ }})
+       -∗ WP Seq (Instr Executable) @ E {{ φ }})%I.
+  Proof.
+    iIntros "%HEheap %HEservice %Hbounds %Hlen".
+    iIntros "(#Hctx & #Hservice & Hna & Hmem & HPC & Hcgp & Hcra & Hca0 & Hca1 & Hca2 & Hct0 & Hct1 & Hct2 & Hct3 & Hct4 & Hctp & Hcnull & Hpost)".
+    (* Open the service invariant and recover the allocator code and state. *)
+    iMod (na_inv_acc with "Hservice Hna") as "(Hinv & Hna & Hclose)"; try exact HEservice.
+    iDestruct "Hinv" as ">[Hstatic Hdata]".
+    iDestruct "Hstatic" as "[Himports Hcode]".
+    iDestruct "Hdata" as (next) "Hdata".
+    iDestruct "Hdata" as "(%Hnext & Hslot & Hroot & Hfree)".
+    (* Use ownership of the range to show that it lies below the bump cursor. *)
+    iMod (allocator_owned_range_below_cursor E b e next ws HEheap Hbounds Hnext Hlen
+      with "Hctx Hmem Hfree") as "(%Hend & Hmem & Hfree)".
+    iAssert (allocator_service_data next) with "[Hslot Hroot Hfree]" as "Hdata".
+    { iFrame. iPureIntro. exact Hnext. }
+    iEval (rewrite /allocator_code) in "Hcode".
+    focus_block_nochangePC 1 "Hcode" as a_free Ha_free "Hfreecode" "Hcode_cont".
+    assert (Ha_eq : a_free = allocator_free_pcc_addr).
+    { pose proof allocator_size_imports as Himports_size.
+      unfold allocator_free_pcc_addr, allocator_free_pcc_off in *. solve_addr. }
+    subst a_free.
+    (* Check the capability and its bounds. *)
+    assert (Hsplit : allocator_free_instrs =
+      (allocator_free_instrs_n 0 ++ allocator_free_instrs_n 1) ++
+      concat (encodeInstrsW <$> drop 2 assembled_allocator_free)) by reflexivity.
+    iEval (rewrite Hsplit) in "Hfreecode".
+    focus_block_0 "Hfreecode" as "Hprepare_code" "Hfree_cont".
+    assert (Hpc : SubBounds allocator_pcc_b allocator_pcc_e
+      allocator_free_pcc_addr (allocator_free_pcc_addr ^+ length allocator_free_instrs)%a).
+    { pose proof allocator_size_code as Hsize_code.
+      rewrite /allocator_code length_app in Hsize_code.
+      unfold allocator_free_pcc_addr, allocator_free_pcc_off in *.
+      solve_addr. }
+    assert (Hdisjoint : disjoint_from_shadow allocator_pcc_b allocator_pcc_e).
+    { pose proof allocator_regions_disjoint as Hregions.
+      unfold disjoint_from_shadow.
+      rewrite !disjoint_list_cons in Hregions.
+      cbn [union_list] in Hregions.
+      set_solver. }
+    iDestruct "Hct0" as (w0) "Hct0".
+    iDestruct "Hct1" as (w1) "Hct1".
+    iDestruct "Hct2" as (w2) "Hct2".
+    iDestruct "Hct3" as (w3) "Hct3".
+    assert (Hrequest : allocator_free_valid next (WCap true p g b e a)).
+    { exists p, g, b, e, a. split; first reflexivity. solve_addr. }
+    iApply (allocator_free_prepare_valid_spec with
+      "[- $Hctx $Hdata $HPC $Hcgp $Hca0 $Hct0 $Hct1 $Hct2 $Hct3 $Hprepare_code]"); eauto.
+    iNext. iIntros "(Hdata & Hcgp & Hca0 & Hprepare_code & Hvalid)".
+    iDestruct "Hvalid" as (p0 g0 b0 e0 a0)
+      "(%Hvalid & HPC & Hct0 & Hct1 & Hct2 & Hct3)".
+    destruct Hvalid as [Heq Hvalid]. inversion Heq; subst; clear Heq.
+    iDestruct ("Hfree_cont" with "Hprepare_code") as "Hfreecode".
+    iEval (rewrite -Hsplit) in "Hfreecode".
+    (* Fetch the shadow capability and translate the range to free. *)
+    assert (Hsplit2 : allocator_free_instrs =
+      concat (encodeInstrsW <$> take 2 assembled_allocator_free) ++
+      (allocator_free_instrs_n 2 ++
+       concat (encodeInstrsW <$> drop 3 assembled_allocator_free))) by reflexivity.
+    iEval (rewrite Hsplit2) in "Hfreecode".
+    focus_block_nochangePC 1 "Hfreecode" as a_fetch Ha_fetch
+      "Hfetch_code" "Hfreecode_cont".
+    assert (Haddr : a_fetch = allocator_free_block_addr allocator_free_pcc_addr 2).
+    { unfold allocator_free_block_addr in *. solve_addr. }
+    subst a_fetch.
+    pose proof allocator_size_imports as Himports_size.
+    iDestruct (region_pointsto_single with "Himports") as (v)
+      "[Himport %Hentry]"; first exact Himports_size.
+    cbn in Hentry. inversion Hentry; subst v.
+    assert (Hfetch_eq : allocator_free_instrs_n 2 =
+      fetch.fetch_instrs allocator_shadow_import_off ctp ct3 ca2)
+      by reflexivity.
+    iEval (rewrite Hfetch_eq) in "Hfetch_code".
+    iDestruct "Hctp" as (wctp) "Hctp".
+    iDestruct "Hca2" as (wca2) "Hca2".
+    assert (Himpaddr : (allocator_pcc_b ^+ allocator_shadow_import_off)%a =
+      allocator_pcc_b) by (unfold allocator_shadow_import_off; solve_addr).
+    iEval (rewrite -Himpaddr) in "Himport".
+    iApply (allocator_fetch_spec with
+      "[- $HPC $Hctp $Hct3 $Hca2 $Hfetch_code $Himport]").
+    { reflexivity. }
+    { rewrite -Hfetch_eq; exact H2. }
+    { apply withinBounds_true_iff; solve_addr. }
+    { exact Hdisjoint. }
+    { cbn [is_heap_cap]; unfold is_heap_address;
+      apply not_true_is_false; intro Hheap;
+      apply withinBounds_true_iff in Hheap;
+      pose proof heap_shadow_disjoint as Hd;
+      rewrite /disjoint_from_shadow elem_of_disjoint in Hd;
+      apply (Hd shadow_b); apply elem_of_finz_seq_between; try exact Hheap;
+      pose proof shadow_valid; solve_addr. }
+    { discriminate. }
+    { discriminate. }
+    { discriminate. }
+    iNext. iIntros "(HPC & Hctp & Hct3 & Hca2 & Hfetch_code & Himport)".
+    iEval (cbn) in "Hctp".
+    iEval (rewrite Himpaddr) in "Himport".
+    iAssert ([[allocator_pcc_b,allocator_code_b]] ↦ₐ [[allocator_imports]])%I
+      with "[Himport]" as "Himports".
+    { rewrite /allocator_imports /region_pointsto
+        (finz_seq_between_singleton allocator_pcc_b allocator_code_b Himports_size) /=.
+      iFrame. }
+    iEval (rewrite -Hfetch_eq) in "Hfetch_code".
+    iDestruct ("Hfreecode_cont" with "Hfetch_code") as "Hfreecode".
+    iEval (rewrite -Hsplit2) in "Hfreecode".
+    assert (Hsplit3 : allocator_free_instrs =
+      concat (encodeInstrsW <$> take 3 assembled_allocator_free) ++
+      (allocator_free_instrs_n 3 ++
+       concat (encodeInstrsW <$> drop 4 assembled_allocator_free))) by reflexivity.
+    iEval (rewrite Hsplit3) in "Hfreecode".
+    focus_block_nochangePC 1 "Hfreecode" as a_translate Ha_translate
+      "Htranslate_code" "Hfreecode_cont".
+    assert (Haddr3 : a_translate =
+      allocator_free_block_addr allocator_free_pcc_addr 3).
+    { unfold allocator_free_block_addr. solve_addr. }
+    subst a_translate.
+    assert (Hpc3 : (allocator_free_block_addr allocator_free_pcc_addr 2 ^+
+      length (fetch.fetch_instrs allocator_shadow_import_off ctp ct3 ca2))%a =
+      allocator_free_block_addr allocator_free_pcc_addr 3).
+    { unfold allocator_free_block_addr. solve_addr. }
+    iEval (rewrite Hpc3) in "HPC".
+    assert (Htranslate_eq : allocator_free_instrs_n 3 =
+      allocator_malloc_instrs_n 4) by reflexivity.
+    iEval (rewrite Htranslate_eq) in "Htranslate_code".
+    iApply (allocator_translate_spec with
+      "[- $HPC $Hct0 $Hct1 $Hct2 $Hct3 $Hctp $Hca2 $Htranslate_code]");
+      eauto; try solve_addr.
+    iNext. iIntros
+      "(HPC & Hct0 & Hct1 & Hct2 & Hct3 & Hctp & Hca2 & Htranslate_code)".
+    iEval (rewrite -Htranslate_eq) in "Htranslate_code".
+    iDestruct ("Hfreecode_cont" with "Htranslate_code") as "Hfreecode".
+    iEval (rewrite -Hsplit3) in "Hfreecode".
+    (* Set the shadow bits and exchange memory ownership for reclaim tokens. *)
+    assert (Hsplit4 : allocator_free_instrs =
+      concat (encodeInstrsW <$> take 4 assembled_allocator_free) ++
+      (allocator_free_instrs_n 4 ++
+       concat (encodeInstrsW <$> drop 5 assembled_allocator_free))) by reflexivity.
+    iEval (rewrite Hsplit4) in "Hfreecode".
+    focus_block_nochangePC 1 "Hfreecode" as a_paint Ha_paint
+      "Hpaint_code" "Hfreecode_cont".
+    assert (Haddr4 : a_paint =
+      allocator_free_block_addr allocator_free_pcc_addr 4).
+    { unfold allocator_free_block_addr. solve_addr. }
+    subst a_paint.
+    assert (Hpc4 : (allocator_free_block_addr allocator_free_pcc_addr 3 ^+
+      length (allocator_malloc_instrs_n 4))%a =
+      allocator_free_block_addr allocator_free_pcc_addr 4).
+    { unfold allocator_free_block_addr. solve_addr. }
+    iEval (rewrite Hpc4) in "HPC".
+    pose (sb := (shadow_b ^+ (b0 - heap_b))%a).
+    pose (se := (shadow_b ^+ (e0 - heap_b))%a).
+    assert (Hshadow : (shadow_b <= sb /\ sb < se /\ se <= shadow_e)%a).
+    { pose proof heap_shadow_same_size. unfold sb, se. solve_addr. }
+    assert (Hlen_shadow : (se - sb = e0 - b0)%Z).
+    { unfold sb, se. pose proof heap_shadow_same_size. solve_addr. }
+    assert (Htranslation : ∀ x, (b0 <= x /\ x < e0)%a ->
+      heap_to_shadow x = Some (sb ^+ (x - b0))%a).
+    { intros x Hx. rewrite allocator_translation_affine.
+      unfold translate_region.
+      assert (Hxheap : withinBounds heap_b heap_e x = true).
+      { apply withinBounds_true_iff. solve_addr. }
+      rewrite Hxheap. unfold sb. pose proof heap_shadow_same_size. solve_addr. }
+    assert (Hpaint_eq : allocator_free_instrs_n 4 =
+      allocator_paint_instrs ctp ca2 true) by reflexivity.
+    iEval (rewrite Hpaint_eq) in "Hpaint_code".
+    iApply (allocator_paint_spec true ctp ca2 E RX Global
+      allocator_pcc_b allocator_pcc_e
+      (allocator_free_block_addr allocator_free_pcc_addr 4) b0 e0 sb se ws
+      with "[- $Hctx $HPC $Hctp $Hca2 $Hpaint_code $Hmem]").
+    { reflexivity. }
+    { rewrite -Hpaint_eq; exact H6. }
+    { exact Hdisjoint. }
+    { exact HEheap. }
+    { solve_addr. }
+    { exact Hshadow. }
+    { exact Hlen_shadow. }
+    { exact Htranslation. }
+    { vm_compute;
+      constructor; [rewrite !elem_of_cons elem_of_nil; intuition congruence|];
+      constructor; [rewrite !elem_of_cons elem_of_nil; intuition congruence|];
+      constructor; [rewrite !elem_of_cons elem_of_nil; intuition congruence|];
+      constructor; [apply not_elem_of_nil|];
+      constructor. }
+    iNext. iIntros "(HPC & Hctp & Hca2 & Hpaint_code & Hreclaimed)".
+    iEval (rewrite -Hpaint_eq) in "Hpaint_code".
+    iDestruct ("Hfreecode_cont" with "Hpaint_code") as "Hfreecode".
+    iEval (rewrite -Hsplit4) in "Hfreecode".
+    (* Set ALLOC_OK, then return and restore the service invariant. *)
+    assert (Hsplit5 : allocator_free_instrs =
+      concat (encodeInstrsW <$> take 5 assembled_allocator_free) ++
+      (allocator_free_instrs_n 5 ++
+       concat (encodeInstrsW <$> drop 6 assembled_allocator_free))) by reflexivity.
+    iEval (rewrite Hsplit5) in "Hfreecode".
+    focus_block_nochangePC 1 "Hfreecode" as a_success Ha_success
+      "Hsuccess_code" "Hfreecode_cont".
+    assert (Haddr5 : a_success =
+      allocator_free_block_addr allocator_free_pcc_addr 5).
+    { unfold allocator_free_block_addr. solve_addr. }
+    subst a_success.
+    assert (Hoff4 : allocator_free_block_addr allocator_free_pcc_addr 4 =
+      (allocator_free_pcc_addr ^+ 32)%a) by reflexivity.
+    assert (Hoff5 : allocator_free_block_addr allocator_free_pcc_addr 5 =
+      (allocator_free_pcc_addr ^+ 36)%a) by reflexivity.
+    assert (Hlenpaint : length (allocator_paint_instrs ctp ca2 true) = 4)
+      by reflexivity.
+    assert (Hpc5 : (allocator_free_block_addr allocator_free_pcc_addr 4 ^+
+       length (allocator_paint_instrs ctp ca2 true))%a =
+       allocator_free_block_addr allocator_free_pcc_addr 5).
+    { clear -Hoff4 Hoff5 Hlenpaint.
+      rewrite Hoff4 Hoff5 Hlenpaint.
+      rewrite incr_addr_opt_add_twice.
+      { replace (32 + 4)%Z with 36%Z by lia; reflexivity. }
+      all: lia. }
+    iEval (rewrite Hpc5) in "HPC".
+    iDestruct "Hca1" as (wca1) "Hca1".
+    iApply (allocator_free_success_block_spec with
+      "[- $HPC $Hca0 $Hca1 $Hsuccess_code]"); eauto.
+    iNext. iIntros "(HPC & Hca0 & Hca1 & Hsuccess_code)".
+    iDestruct ("Hfreecode_cont" with "Hsuccess_code") as "Hfreecode".
+    iEval (rewrite -Hsplit5) in "Hfreecode".
+    assert (Hsplit7 : allocator_free_instrs =
+      concat (encodeInstrsW <$> take 7 assembled_allocator_free) ++
+      allocator_free_instrs_n 7) by reflexivity.
+    iEval (rewrite Hsplit7) in "Hfreecode".
+    focus_block_nochangePC 1 "Hfreecode" as a_ret Ha_ret
+      "Hret_code" "Hfreecode_cont".
+    assert (Haddr7 : a_ret =
+      allocator_free_block_addr allocator_free_pcc_addr 7).
+    { unfold allocator_free_block_addr. clear -Ha_ret.
+      cbn [take concat fmap] in *. solve_addr. }
+    subst a_ret.
+    assert (Hret_eq : allocator_free_instrs_n 7 =
+      encodeInstrsW [Jalr cnull cra]) by reflexivity.
+    iEval (rewrite Hret_eq) in "Hret_code".
+    iDestruct "Hcnull" as (wnull) "Hcnull".
+    iApply (allocator_return_spec with
+      "[- $HPC $Hcra $Hcnull $Hret_code]"); eauto.
+    iNext. iIntros "(HPC & Hcra & Hcnull & Hret_code)".
+    iEval (rewrite -Hret_eq) in "Hret_code".
+    iDestruct ("Hfreecode_cont" with "Hret_code") as "Hfreecode".
+    iEval (rewrite -Hsplit7) in "Hfreecode".
+    iDestruct ("Hcode_cont" with "Hfreecode") as "Hcode".
+    iEval (rewrite -/allocator_code) in "Hcode".
+    iMod ("Hclose" with "[Himports Hcode Hdata Hna]") as "Hna".
+    { iSplitR "Hna"; last iFrame.
+      iNext. iSplitL "Himports Hcode"; first iFrame.
+      iExists next. iFrame. }
+    iApply "Hpost". iFrame "∗".
+  Qed.
+End AllocatorFreeProof.
