theories/allocator/allocator_macros_spec.v
@@ -1,0 +1,384 @@
+From iris.proofmode Require Import proofmode.
+From griotte Require Import rules proofmode memory_region fetch.
+From griotte.allocator Require Import allocator_preamble.
+
+(** Loop specifications. Fetch and return use the existing instruction/macro rules.
+    Every loop requires a nonempty range because it stores before testing.
+    Registers not mentioned in the contracts can be framed. *)
+Section AllocatorMacros.
+  Context
+    {Σ : gFunctors}
+    {ceriseg : ceriseG Σ}
+    {allocatorg : allocatorG Σ}
+    {MP : MachineParameters}
+  .
+
+  (** The existing fetch macro proof specialized to an arbitrary WP mask, so
+      allocator calls can keep the non-atomic service invariant open. *)
+  Lemma allocator_fetch_spec
+    (n : Z) (rdst rscratch1 rscratch2 : RegName) (E : coPset)
+    (pc_p : Perm) (pc_g : Locality) (pc_b pc_e pc_a : Addr)
+    (wentry wdst w1 w2 : Word)
+    (φ : language.val griotte_lang → iPropI Σ) :
+
+    let code := fetch_instrs n rdst rscratch1 rscratch2 in
+    let pc_end := (pc_a ^+ length code)%a in
+    executeAllowed pc_p = true ->
+    SubBounds pc_b pc_e pc_a pc_end ->
+    withinBounds pc_b pc_e (pc_b ^+ n)%a = true ->
+    disjoint_from_shadow pc_b pc_e ->
+    is_heap_cap wentry = false ->
+    rdst ≠ cnull ->
+    rscratch1 ≠ cnull ->
+    rscratch2 ≠ cnull ->
+
+    ▷ PC ↦ᵣ WCap true pc_p pc_g pc_b pc_e pc_a
+    ∗ ▷ rdst ↦ᵣ wdst
+    ∗ ▷ rscratch1 ↦ᵣ w1
+    ∗ ▷ rscratch2 ↦ᵣ w2
+    ∗ ▷ codefrag pc_a code
+    ∗ ▷ (pc_b ^+ n)%a ↦ₐ wentry
+    ∗ ▷ (PC ↦ᵣ WCap true pc_p pc_g pc_b pc_e pc_end
+         ∗ rdst ↦ᵣ load_word pc_p wentry
+         ∗ rscratch1 ↦ᵣ WInt 0
+         ∗ rscratch2 ↦ᵣ WInt 0
+         ∗ codefrag pc_a code
+         ∗ (pc_b ^+ n)%a ↦ₐ wentry
+         -∗ WP Seq (Instr Executable) @ E {{ φ }})
+    ⊢ WP Seq (Instr Executable) @ E {{ φ }}.
+  Proof.
+    intros code pc_end Hvpc Hcont Hpc_n Hdisjoint Hnonheap Hrdst Hr1 Hr2;
+      subst code pc_end.
+    iIntros "(>HPC & >Hrdst & >Hscratch1 & >Hscratch2 & >Hcode & >Hentry & Hφ)".
+    codefrag_facts "Hcode".
+    assert ((pc_a + (pc_b - pc_a))%a = Some pc_b) as Hlea by solve_addr.
+    assert ((pc_b + n)%a = Some (pc_b ^+ n)%a) as Hpc_bn by solve_addr.
+    assert (is_shadow_address (pc_b ^+ n)%a = false) as Hshadow.
+    { eapply disjoint_from_shadow_not_in; eauto. }
+    iGo "Hcode".
+    iApply "Hφ"; iFrame.
+  Qed.
+
+  Lemma allocator_return_spec
+    (E : coPset) (pc_b pc_e pc_a : Addr) (wret wnull : Word)
+    (φ : language.val griotte_lang → iPropI Σ) :
+
+    let code := encodeInstrsW [Jalr cnull cra] in
+    SubBounds pc_b pc_e pc_a (pc_a ^+ length code)%a ->
+    disjoint_from_shadow pc_b pc_e ->
+
+    ▷ PC ↦ᵣ WCap true RX Global pc_b pc_e pc_a
+    ∗ ▷ cra ↦ᵣ wret
+    ∗ ▷ cnull ↦ᵣ wnull
+    ∗ ▷ codefrag pc_a code
+    ∗ ▷ (PC ↦ᵣ updatePcPerm wret
+         ∗ cra ↦ᵣ wret
+         ∗ cnull ↦ᵣ WInt 0
+         ∗ codefrag pc_a code
+         -∗ WP Seq (Instr Executable) @ E {{ φ }})
+    ⊢ WP Seq (Instr Executable) @ E {{ φ }}.
+  Proof.
+    intros code Hpc Hdisjoint; subst code.
+    iIntros "(>HPC & >Hcra & >Hcnull & >Hcode & Hφ)".
+    codefrag_facts "Hcode".
+    (* Jalr cnull cra. *)
+    iInstr "Hcode".
+    iApply "Hφ". iFrame.
+  Qed.
+
+  Lemma allocator_zero_spec
+    (rptr rend rtmp : RegName) (E : coPset)
+    (pc_p : Perm) (pc_g : Locality) (pc_b pc_e pc_a : Addr)
+    (p : Perm) (g : Locality) (b e : Addr) (wtmp : Word)
+    (φ : language.val griotte_lang → iPropI Σ) :
+
+    let code := allocator_zero_instrs rptr rend rtmp in
+    let pc_end := (pc_a ^+ length code)%a in
+    executeAllowed pc_p = true ->
+    SubBounds pc_b pc_e pc_a pc_end ->
+    disjoint_from_shadow pc_b pc_e ->
+    writeAllowed p = true ->
+    (heap_b <= b /\ b < e /\ e <= heap_e)%a ->
+    NoDup [PC; cnull; rptr; rend; rtmp] ->
+
+    ▷ PC ↦ᵣ WCap true pc_p pc_g pc_b pc_e pc_a
+    ∗ ▷ rptr ↦ᵣ WCap true p g b e b
+    ∗ ▷ rend ↦ᵣ WInt (finz.to_z e)
+    ∗ ▷ rtmp ↦ᵣ wtmp
+    ∗ ▷ codefrag pc_a code
+    ∗ ▷ allocator_range_memory b e
+    ∗ ▷ (PC ↦ᵣ WCap true pc_p pc_g pc_b pc_e pc_end
+         ∗ rptr ↦ᵣ WCap true p g b e e
+         ∗ rend ↦ᵣ WInt (finz.to_z e)
+         ∗ rtmp ↦ᵣ WInt 0
+         ∗ codefrag pc_a code
+         ∗ ([∗ list] a ∈ finz.seq_between b e, a ↦ₐ WInt 0)
+         -∗ WP Seq (Instr Executable) @ E {{ φ }})
+    ⊢ WP Seq (Instr Executable) @ E {{ φ }}.
+
+  Proof.
+    intros code pc_end; subst code pc_end.
+    iIntros (Hexec Hpc Hpc_shadow Hwrite Hheap Hregs)
+      "(>HPC & >Hptr & >Hend & >Htmp & >Hcode & >Hmem & Hφ)".
+    assert (Hrptr : rptr ≠ cnull) by (repeat rewrite NoDup_cons in Hregs; set_solver).
+    assert (Hrend : rend ≠ cnull) by (repeat rewrite NoDup_cons in Hregs; set_solver).
+    assert (Hrtmp : rtmp ≠ cnull) by (repeat rewrite NoDup_cons in Hregs; set_solver).
+
+    (* Keep the capability's base fixed while the loop cursor advances. *)
+    pose (cap_b := b).
+    assert (Hcap_b : (heap_b <= cap_b)%a) by (unfold cap_b; solve_addr).
+    assert (Hba : (cap_b <= b)%a) by (unfold cap_b; solve_addr).
+    assert (Hbase : b = cap_b) by done.
+    iEval (rewrite {1}Hbase) in "Hptr".
+    iEval (rewrite {1}Hbase) in "Hφ".
+    clear Hbase; clearbody cap_b.
+    iLöb as "IH" forall (b wtmp Hheap Hba).
+    codefrag_facts "Hcode".
+    iEval (rewrite /allocator_range_memory
+      (finz_seq_between_cons b e (proj1 (proj2 Hheap))) big_sepL_cons) in "Hmem".
+    iDestruct "Hmem" as "[[%w Ha] Hmem]".
+
+    (* Store rptr 0 writes zero to the current heap cell. *)
+    iInstr_lookup "Hcode" as "Hi" "Hcode".
+    wp_instr.
+    iApply (wp_store_success_z with "[$HPC $Hi $Hptr $Ha]"); try solve_pure.
+    { eapply disjoint_from_shadow_not_in; first exact heap_shadow_disjoint.
+      apply withinBounds_true_iff; solve_addr. }
+    { apply withinBounds_true_iff; solve_addr. }
+    iIntros "!> (HPC & Hi & Hptr & Ha)".
+    wp_pure.
+    iSpecialize ("Hcode" with "Hi").
+
+    (* Lea rptr 1 advances the heap cursor. *)
+    iInstr "Hcode".
+    (* GetA rtmp rptr reads the advanced cursor. *)
+    iInstr "Hcode".
+    (* Sub rtmp rend rtmp computes the remaining length. *)
+    iInstr "Hcode".
+    destruct (decide ((b ^+ 1)%a = e)) as [Hlast | Hmore].
+    - rewrite Hlast Z.sub_diag.
+      (* Jnz .allocator_zero rtmp falls through after the last cell. *)
+      iInstr "Hcode".
+      iApply "Hφ"; iFrame.
+      rewrite (finz_seq_between_cons b e (proj1 (proj2 Hheap)))
+        Hlast finz_seq_between_empty; last solve_addr.
+      rewrite big_sepL_cons big_sepL_nil. iFrame.
+    - (* Jnz .allocator_zero rtmp repeats the loop. *)
+      iInstr_lookup "Hcode" as "Hi" "Hcode".
+      wp_instr.
+      iApply (wp_jnz_success_jmp_z with "[$HPC $Hi $Htmp]"); try solve_pure.
+      { intros Hzero; inversion Hzero; solve_addr. }
+      { instantiate (1 := pc_a). solve_addr. }
+      iIntros "!> (HPC & Hi & Htmp)".
+      wp_pure.
+      iSpecialize ("Hcode" with "Hi").
+      iApply ("IH" $! (b ^+ 1)%a with
+        "[] [] HPC Hptr Hend Htmp Hcode Hmem [Ha Hφ]").
+      { iPureIntro; solve_addr. }
+      { iPureIntro; solve_addr. }
+      iNext. iIntros "(HPC & Hptr & Hend & Htmp & Hcode & Hzero)".
+      iApply "Hφ"; iFrame.
+      rewrite (finz_seq_between_cons b e (proj1 (proj2 Hheap))) big_sepL_cons.
+      iFrame.
+  Qed.
+
+  (** Clear painting preserves the exact words supplied by the caller.
+      Quarantine painting gives up those words and returns one reclaim token
+      per cell. In either case, memory ownership witnesses that the entire
+      input range is live; repeated runtime frees are outside this contract.
+
+      The translation and length premises identify the shadow interval, including
+      the one-past-end pointer reached by the final LEA but never dereferenced.
+      The service layout supplies them when composing the allocator operations. *)
+  Lemma allocator_paint_spec
+    (bit : bool) (rptr rcount : RegName) (E : coPset)
+    (pc_p : Perm) (pc_g : Locality) (pc_b pc_e pc_a : Addr)
+    (b e sb se : Addr) (ws : list Word)
+    (φ : language.val griotte_lang → iPropI Σ) :
+
+    let code := allocator_paint_instrs rptr rcount bit in
+    let pc_end := (pc_a ^+ length code)%a in
+    executeAllowed pc_p = true ->
+    SubBounds pc_b pc_e pc_a pc_end ->
+    disjoint_from_shadow pc_b pc_e ->
+    ↑Nallocator ⊆ E ->
+    (heap_b <= b /\ b < e /\ e <= heap_e)%a ->
+    (shadow_b <= sb /\ sb < se /\ se <= shadow_e)%a ->
+    (finz.to_z se - finz.to_z sb = finz.to_z e - finz.to_z b)%Z ->
+    (∀ a, (b <= a /\ a < e)%a ->
+       heap_to_shadow a = Some (sb ^+ (finz.to_z a - finz.to_z b))%a) ->
+    NoDup [PC; cnull; rptr; rcount] ->
+
+    allocator_ctx
+    ∗ ▷ PC ↦ᵣ WCap true pc_p pc_g pc_b pc_e pc_a
+    ∗ ▷ rptr ↦ᵣ WCap true RW Global shadow_b shadow_e sb
+    ∗ ▷ rcount ↦ᵣ WInt (finz.to_z e - finz.to_z b)
+    ∗ ▷ codefrag pc_a code
+    ∗ ▷ ([[b, e]] ↦ₐ [[ws]])
+    ∗ ▷ (PC ↦ᵣ WCap true pc_p pc_g pc_b pc_e pc_end
+         ∗ rptr ↦ᵣ WCap true RW Global shadow_b shadow_e se
+         ∗ rcount ↦ᵣ WInt 0
+         ∗ codefrag pc_a code
+         ∗ (if bit then [∗ list] a ∈ finz.seq_between b e, reclaim_token a
+            else [[b, e]] ↦ₐ [[ws]])
+         -∗ WP Seq (Instr Executable) @ E {{ φ }})
+    ⊢ WP Seq (Instr Executable) @ E {{ φ }}.
+  Proof.
+    intros code pc_end; subst code pc_end.
+    iIntros (Hexec Hpc Hpc_shadow HE Hheap Hshadow Hlen Htranslate Hregs)
+      "(#Halloc & >HPC & >Hptr & >Hcount & >Hcode & >Hmem & Hφ)".
+    assert (Hrptr : rptr ≠ cnull) by
+      (clear -Hregs; repeat rewrite NoDup_cons in Hregs; set_solver).
+    assert (Hrcount : rcount ≠ cnull) by
+      (clear -Hregs; repeat rewrite NoDup_cons in Hregs; set_solver).
+    iLöb as "IH" forall (b sb ws Hheap Hshadow Hlen Htranslate).
+    assert (Hcode_eq : allocator_paint_instrs rptr rcount bit =
+      encodeInstrsW [Store rptr (inl (bool_to_Z bit)) 0;
+                    Lea rptr (inl 1%Z);
+                    Sub rcount (inr rcount) (inl 1%Z);
+                    Jnz (inl (-3)%Z) rcount]) by (destruct bit; reflexivity).
+    rewrite Hcode_eq in Hpc |- *.
+    codefrag_facts "Hcode".
+    iDestruct (big_sepL2_length with "Hmem") as %Hws.
+    rewrite (finz_seq_between_cons b e (proj1 (proj2 Hheap))) in Hws.
+    clear Hcode_eq.
+    destruct ws as [|w ws]; first discriminate Hws.
+    assert (Hbnext : (b + 1)%a = Some (b ^+ 1)%a) by solve_addr.
+    assert (Hbnext_e : (b ^+ 1 <= e)%a) by solve_addr.
+    iEval (rewrite (region_pointsto_cons b (b ^+ 1)%a e w ws Hbnext Hbnext_e))
+      in "Hmem".
+    iDestruct "Hmem" as "[Ha Hmem]".
+    assert (Hmap : heap_to_shadow b = Some sb).
+    { specialize (Htranslate b).
+      replace (sb ^+ (b - b))%a with sb in Htranslate by solve_addr.
+      apply Htranslate; solve_addr. }
+
+    (* Store rptr bit writes the shadow entry, opening the shared invariant. *)
+    iInstr_lookup "Hcode" as "Hi" "Hcode".
+    wp_instr.
+    iAssert (WP Instr Executable @ E {{ v,
+      ⌜v = NextIV⌝ ∗
+      PC ↦ᵣ WCap true pc_p pc_g pc_b pc_e (pc_a ^+ 1)%a ∗
+      pc_a ↦ₐ encodeInstrW (Store rptr (inl (bool_to_Z bit)) 0) ∗
+      rptr ↦ᵣ WCap true RW Global shadow_b shadow_e sb ∗
+      (if bit then reclaim_token b else b ↦ₐ w) }})%I
+      with "[HPC Hi Hptr Ha]" as "Hstore".
+    { iApply (wp_atomic _ _ (E ∖ ↑Nallocator)).
+      iInv Nallocator as ">Hbody" "Hclose".
+      iDestruct (allocator_inv_lookup b with "Hbody") as (s) "[Hentry Hput]".
+      { apply elem_of_heap_addresses, withinBounds_true_iff; solve_addr. }
+      iDestruct (allocator_entry_memory_live with "Hentry Ha") as %->.
+      iDestruct "Hentry" as "[Hs [Hreclaim Hfree]]".
+      iModIntro.
+      iApply (wp_store_success_shadow_z _ _ _ _ _ _ _ _ _ _ _ _ _ _ bit false
+        with "[$HPC $Hi $Hptr $Hs]"); try solve_pure.
+      { unfold is_shadow_address. apply withinBounds_true_iff; solve_addr. }
+      { by apply heap_shadow_inverse. }
+      { apply withinBounds_true_iff; solve_addr. }
+      iIntros "!> (HPC & Hi & Hptr & Hs)".
+      destruct bit.
+      - iMod ("Hclose" with "[Ha Hs Hput Hfree]").
+        { iNext. iApply ("Hput" $! Quarantined). iFrame. }
+        iModIntro; iFrame; done.
+      - iMod ("Hclose" with "[Hs Hput Hfree Hreclaim]").
+        { iNext. iApply ("Hput" $! Live). iFrame. }
+        iModIntro; iFrame; done.
+    }
+    iApply (wp_wand with "Hstore").
+    iIntros (v) "(-> & HPC & Hi & Hptr & Ha)".
+    wp_pure.
+    iSpecialize ("Hcode" with "Hi").
+
+    (* Lea rptr 1 advances the shadow cursor. *)
+    iInstr "Hcode".
+    (* Sub rcount rcount 1 consumes one word of the count. *)
+    iInstr "Hcode".
+    destruct (decide ((b ^+ 1)%a = e)) as [Hlast | Hmore].
+    - replace (e - b - 1)%Z with 0%Z by solve_addr.
+      (* Jnz .allocator_paint rcount falls through after the last cell. *)
+      iInstr "Hcode".
+      assert (Hslast : (sb ^+ 1)%a = se) by solve_addr.
+      rewrite Hslast.
+      iApply "Hφ"; iFrame.
+      destruct bit.
+      + rewrite (finz_seq_between_cons b e (proj1 (proj2 Hheap)))
+          Hlast finz_seq_between_empty; last solve_addr.
+        rewrite big_sepL_cons big_sepL_nil. iFrame.
+      + rewrite (region_pointsto_cons b (b ^+ 1)%a e w ws Hbnext Hbnext_e).
+        iFrame.
+    - (* Jnz .allocator_paint rcount repeats the loop. *)
+      iInstr_lookup "Hcode" as "Hi" "Hcode".
+      wp_instr.
+      iApply (wp_jnz_success_jmp_z with "[$HPC $Hi $Hcount]"); try solve_pure.
+      { intros Hzero; inversion Hzero; solve_addr. }
+      { instantiate (1 := pc_a). solve_addr. }
+      iIntros "!> (HPC & Hi & Hcount)".
+      wp_pure.
+      iSpecialize ("Hcode" with "Hi").
+      replace (e - b - 1)%Z with (e - (b ^+ 1)%a)%Z by solve_addr.
+      iApply ("IH" $! (b ^+ 1)%a (sb ^+ 1)%a ws with
+        "[] [] [] [] HPC Hptr Hcount Hcode Hmem [Ha Hφ]").
+      { iPureIntro; solve_addr. }
+      { iPureIntro; solve_addr. }
+      { iPureIntro; solve_addr. }
+      { iPureIntro. intros a Ha_bounds.
+        rewrite (Htranslate a); last solve_addr.
+        f_equal. clear -Hheap Hshadow Hlen Hbnext Ha_bounds. solve_addr. }
+      iNext. iIntros "(HPC & Hptr & Hcount & Hcode & Hpainted)".
+      iApply "Hφ"; iFrame.
+      destruct bit.
+      + rewrite (finz_seq_between_cons b e (proj1 (proj2 Hheap))) big_sepL_cons.
+        iFrame.
+      + rewrite (region_pointsto_cons b (b ^+ 1)%a e w ws Hbnext Hbnext_e).
+        iFrame.
+  Qed.
+  (** Translate a heap interval to its shadow interval. The instruction list
+      is shared by malloc block 4 and free block 3. *)
+  Lemma allocator_translate_spec
+    (E : coPset)
+    (pc_b pc_e pc_a next b e : Addr) (w3 wa2 : Word)
+    (φ : language.val griotte_lang → iPropI Σ) :
+
+    let code := allocator_malloc_instrs_n 4 in
+    let sb := (shadow_b ^+ (b - heap_b))%a in
+    SubBounds pc_b pc_e pc_a (pc_a ^+ length code)%a ->
+    disjoint_from_shadow pc_b pc_e ->
+    (heap_b <= b /\ b < e /\ e <= heap_e)%a ->
+
+    ▷ PC ↦ᵣ WCap true RX Global pc_b pc_e pc_a
+    ∗ ▷ ct0 ↦ᵣ WCap true RW Global heap_b heap_e next
+    ∗ ▷ ct1 ↦ᵣ WInt b
+    ∗ ▷ ct2 ↦ᵣ WInt e
+    ∗ ▷ ct3 ↦ᵣ w3
+    ∗ ▷ ctp ↦ᵣ WCap true RW Global shadow_b shadow_e shadow_b
+    ∗ ▷ ca2 ↦ᵣ wa2
+    ∗ ▷ codefrag pc_a code
+    ∗ ▷ (PC ↦ᵣ WCap true RX Global pc_b pc_e (pc_a ^+ length code)%a
+         ∗ ct0 ↦ᵣ WCap true RW Global heap_b heap_e next
+         ∗ ct1 ↦ᵣ WInt b
+         ∗ ct2 ↦ᵣ WInt e
+         ∗ ct3 ↦ᵣ WInt (b - heap_b)
+         ∗ ctp ↦ᵣ WCap true RW Global shadow_b shadow_e sb
+         ∗ ca2 ↦ᵣ WInt (e - b)
+         ∗ codefrag pc_a code
+         -∗ WP Seq (Instr Executable) @ E {{ φ }})
+    ⊢ WP Seq (Instr Executable) @ E {{ φ }}.
+
+  Proof.
+    intros code sb Hpc Hdisjoint Hheap; subst code sb.
+    iIntros "(>HPC & >Hct0 & >Hct1 & >Hct2 & >Hct3 & >Hctp & >Hca2 & >Hcode & Hφ)".
+    codefrag_facts "Hcode".
+    (* GetB ct3 ct0. *)
+    iInstr "Hcode".
+    (* Sub ct3 ct1 ct3. *)
+    iInstr "Hcode".
+    pose proof heap_shadow_same_size as Hsize.
+    assert (Hsb : (shadow_b <= (shadow_b ^+ (b - heap_b))%a /\
+                   (shadow_b ^+ (b - heap_b))%a < shadow_e)%a) by solve_addr.
+    (* Lea ctp ct3. *)
+    iInstr "Hcode".
+    (* Sub ca2 ct2 ct1. *)
+    iInstr "Hcode".
+    iApply "Hφ". iFrame.
+  Qed.
+End AllocatorMacros.
