theories/allocator/allocator_malloc_spec.v
@@ -1,0 +1,1146 @@
+From iris.proofmode Require Import proofmode.
+From griotte Require Import rules proofmode memory_region.
+From griotte.allocator Require Import allocator_preamble
+  allocator_macros_spec allocator_resource_spec.
+
+(** Address of an assembled block relative to the entry point. *)
+Definition allocator_malloc_block_addr {MP : MachineParameters}
+  (pc_a : Addr) (n : nat) : Addr :=
+  (pc_a ^+ length (concat (take n assembled_allocator_malloc)))%a.
+
+Section AllocatorMallocBlocks.
+  Context {Σ : gFunctors} {ceriseg : ceriseG Σ} {allocatorg : allocatorG Σ}
+    {MP : MachineParameters} {layout : allocatorLayout}.
+
+  Lemma allocator_malloc_size_check_valid_spec
+    (E : coPset)
+    (pc_b pc_e pc_a : Addr) (wreq wtmp : Word)
+    (φ : language.val griotte_lang → iPropI Σ) :
+
+    let code := allocator_malloc_instrs_n 0 in
+    ContiguousRegion pc_a (length allocator_malloc_instrs) ->
+    SubBounds pc_b pc_e pc_a (pc_a ^+ length allocator_malloc_instrs)%a ->
+    disjoint_from_shadow pc_b pc_e ->
+    allocator_positive_size wreq ->
+
+    ▷ PC ↦ᵣ WCap true RX Global pc_b pc_e pc_a
+    ∗ ▷ ca0 ↦ᵣ wreq
+    ∗ ▷ ct3 ↦ᵣ wtmp
+    ∗ ▷ codefrag pc_a code
+    ∗ ▷ (ca0 ↦ᵣ wreq
+         ∗ ct3 ↦ᵣ -
+         ∗ codefrag pc_a code
+         ∗ PC ↦ᵣ WCap true RX Global pc_b pc_e
+             (allocator_malloc_block_addr pc_a 1)
+         -∗ WP Seq (Instr Executable) @ E {{ φ }})
+    ⊢ WP Seq (Instr Executable) @ E {{ φ }}.
+  Proof.
+    intros code Hcont Hpc Hdisjoint (n & -> & Hpositive); subst code.
+    iIntros "(>HPC & >Hca0 & >Hct3 & >Hcode & Hφ)".
+    codefrag_facts "Hcode".
+    (* GetWType ct3 ca0. *)
+    iInstr "Hcode".
+    (* Sub ct3 ct3 (encodeWordType wt_int). *)
+    iInstr "Hcode".
+    rewrite (encodeWordType_correct_int n 0) /wt_int Z.sub_diag.
+    (* Jnz .malloc_invalid ct3 falls through for an integer. *)
+    iInstr "Hcode".
+    (* Lt ct3 0 ca0. *)
+    iInstr "Hcode".
+    replace (0 <? n)%Z with true by (symmetry; apply Z.ltb_lt; lia).
+    (* Jnz .malloc_size_ok ct3. *)
+    iInstr "Hcode".
+    iApply "Hφ". iFrame.
+  Qed.
+
+  Lemma allocator_malloc_size_check_invalid_spec
+    (E : coPset)
+    (pc_b pc_e pc_a : Addr) (wreq wtmp : Word)
+    (φ : language.val griotte_lang → iPropI Σ) :
+
+    let code := allocator_malloc_instrs_n 0 in
+    ContiguousRegion pc_a (length allocator_malloc_instrs) ->
+    SubBounds pc_b pc_e pc_a (pc_a ^+ length allocator_malloc_instrs)%a ->
+    disjoint_from_shadow pc_b pc_e ->
+    ¬ allocator_positive_size wreq ->
+
+    ▷ PC ↦ᵣ WCap true RX Global pc_b pc_e pc_a
+    ∗ ▷ ca0 ↦ᵣ wreq
+    ∗ ▷ ct3 ↦ᵣ wtmp
+    ∗ ▷ codefrag pc_a code
+    ∗ ▷ (ca0 ↦ᵣ wreq
+         ∗ ct3 ↦ᵣ -
+         ∗ codefrag pc_a code
+         ∗ PC ↦ᵣ WCap true RX Global pc_b pc_e
+             (allocator_malloc_block_addr pc_a 7)
+         -∗ WP Seq (Instr Executable) @ E {{ φ }})
+    ⊢ WP Seq (Instr Executable) @ E {{ φ }}.
+  Proof.
+    intros code Hcont Hpc Hdisjoint Hinvalid; subst code.
+    iIntros "(>HPC & >Hca0 & >Hct3 & >Hcode & Hφ)".
+    codefrag_facts "Hcode".
+    (* GetWType ct3 ca0. *)
+    iInstr "Hcode".
+    (* Sub ct3 ct3 (encodeWordType wt_int). *)
+    iInstr "Hcode".
+    destruct (is_z wreq) eqn:Hreq_z.
+    - destruct wreq; cbn in *; try done.
+      rewrite (encodeWordType_correct_int z 0) /wt_int Z.sub_diag.
+      (* Jnz .malloc_invalid ct3 falls through for an integer. *)
+      iInstr "Hcode".
+      (* Lt ct3 0 ca0. *)
+      iInstr "Hcode".
+      destruct (decide (0 < z)%Z) as [Hzpos|Hznonpos].
+      { exfalso. apply Hinvalid. exists z. split; [reflexivity|exact Hzpos]. }
+      replace (0 <? z)%Z with false by (symmetry; apply Z.ltb_ge; lia).
+      (* Jnz .malloc_size_ok ct3 falls through. *)
+      iInstr "Hcode".
+      (* Jmp .malloc_invalid leaves this block's code fragment. *)
+      iInstr "Hcode".
+      iApply "Hφ". iFrame.
+    - assert (Hnonzero : WInt (encodeWordType wreq - encodeWordType (WInt 0)) ≠ WInt 0).
+      { pose proof (encodeWordType_correct wreq (WInt 0)) as Hencode.
+        intro Hzero. injection Hzero as Hzero.
+        assert (Heq : encodeWordType wreq = encodeWordType (WInt 0)) by lia.
+        destruct wreq; cbn in Hreq_z, Hencode; try discriminate.
+        all: try (destruct sb; cbn in Hencode); contradiction. }
+      (* Jnz .malloc_invalid ct3 leaves this block's code fragment. *)
+      iInstr "Hcode".
+      iApply "Hφ". iFrame.
+  Qed.
+
+  Lemma allocator_malloc_reject_block_spec
+    (E : coPset) (pc_b pc_e pc_a : Addr) (wreq wstatus : Word)
+    (φ : language.val griotte_lang → iPropI Σ) :
+
+    let start := allocator_malloc_block_addr pc_a 7 in
+    let code := allocator_malloc_instrs_n 7 in
+    ContiguousRegion pc_a (length allocator_malloc_instrs) ->
+    SubBounds pc_b pc_e pc_a (pc_a ^+ length allocator_malloc_instrs)%a ->
+    disjoint_from_shadow pc_b pc_e ->
+
+    ▷ PC ↦ᵣ WCap true RX Global pc_b pc_e start
+    ∗ ▷ ca0 ↦ᵣ wreq
+    ∗ ▷ ca1 ↦ᵣ wstatus
+    ∗ ▷ codefrag start code
+    ∗ ▷ (PC ↦ᵣ WCap true RX Global pc_b pc_e
+           (allocator_malloc_block_addr pc_a 9)
+         ∗ ca0 ↦ᵣ WInt 0
+         ∗ ca1 ↦ᵣ WInt ALLOC_INVALID
+         ∗ codefrag start code
+         -∗ WP Seq (Instr Executable) @ E {{ φ }})
+    ⊢ WP Seq (Instr Executable) @ E {{ φ }}.
+  Proof.
+    intros start code Hcont Hpc Hshadow; subst start code.
+    iIntros "(>HPC & >Hca0 & >Hca1 & >Hcode & Hφ)".
+    codefrag_facts "Hcode".
+    (* Mov ca0 0. *)
+    iInstr "Hcode".
+    assert (Hstep : (pc_a ^+ 44)%a =
+      ((allocator_malloc_block_addr pc_a 7) ^+ 1)%a).
+    { unfold allocator_malloc_block_addr. solve_addr. }
+    iEval (rewrite Hstep) in "HPC".
+    (* Mov ca1 ALLOC_INVALID. *)
+    iInstr "Hcode".
+    iEval (simpl) in "Hca1".
+    (* Jmp .malloc_return. *)
+    iInstr "Hcode".
+    assert (Hca1val :
+      (if decide (ca1 = cnull) then 0%Z else (-1)%Z) = ALLOC_INVALID).
+    { unfold ALLOC_INVALID.
+      destruct (decide (ca1 = cnull)); [discriminate|done]. }
+    iEval (rewrite Hca1val) in "Hca1".
+    assert (Hret : (allocator_malloc_block_addr pc_a 7 ^+ 5)%a =
+      allocator_malloc_block_addr pc_a 9).
+    { unfold allocator_malloc_block_addr. solve_addr. }
+    iEval (rewrite Hret) in "HPC".
+    iApply "Hφ". iFrame.
+  Qed.
+
+  Lemma allocator_malloc_oom_block_spec
+    (E : coPset) (pc_b pc_e pc_a : Addr) (wreq wstatus : Word)
+    (φ : language.val griotte_lang → iPropI Σ) :
+
+    let start := allocator_malloc_block_addr pc_a 8 in
+    let code := allocator_malloc_instrs_n 8 in
+    ContiguousRegion pc_a (length allocator_malloc_instrs) ->
+    SubBounds pc_b pc_e pc_a (pc_a ^+ length allocator_malloc_instrs)%a ->
+    disjoint_from_shadow pc_b pc_e ->
+
+    ▷ PC ↦ᵣ WCap true RX Global pc_b pc_e start
+    ∗ ▷ ca0 ↦ᵣ wreq
+    ∗ ▷ ca1 ↦ᵣ wstatus
+    ∗ ▷ codefrag start code
+    ∗ ▷ (PC ↦ᵣ WCap true RX Global pc_b pc_e
+           (allocator_malloc_block_addr pc_a 9)
+         ∗ ca0 ↦ᵣ WInt 0
+         ∗ ca1 ↦ᵣ WInt ALLOC_NO_MEMORY
+         ∗ codefrag start code
+         -∗ WP Seq (Instr Executable) @ E {{ φ }})
+    ⊢ WP Seq (Instr Executable) @ E {{ φ }}.
+  Proof.
+    intros start code Hcont Hpc Hshadow; subst start code.
+    iIntros "(>HPC & >Hca0 & >Hca1 & >Hcode & Hφ)".
+    codefrag_facts "Hcode".
+    (* Mov ca0 0. *)
+    iInstr "Hcode".
+    assert (Hstep : (pc_a ^+ 47)%a =
+      ((allocator_malloc_block_addr pc_a 8) ^+ 1)%a).
+    { unfold allocator_malloc_block_addr. solve_addr. }
+    iEval (rewrite Hstep) in "HPC".
+    (* Mov ca1 ALLOC_NO_MEMORY. *)
+    iInstr "Hcode".
+    assert (Hca1val :
+      (if decide (ca1 = cnull) then 0%Z else (-2)%Z) = ALLOC_NO_MEMORY).
+    { unfold ALLOC_NO_MEMORY.
+      destruct (decide (ca1 = cnull)); [discriminate|done]. }
+    iEval (rewrite Hca1val) in "Hca1".
+    assert (Hret : (allocator_malloc_block_addr pc_a 8 ^+ 2)%a =
+      allocator_malloc_block_addr pc_a 9).
+    { unfold allocator_malloc_block_addr. solve_addr. }
+    iEval (rewrite Hret) in "HPC".
+    iApply "Hφ". iFrame.
+  Qed.
+
+  Lemma allocator_malloc_prepare_success_spec
+    (E : coPset)
+    (pc_b pc_e pc_a next : Addr) (n : Z)
+    (w0 w1 w2 w3 w4 wa2 : Word)
+    (φ : language.val griotte_lang → iPropI Σ) :
+
+    let start := allocator_malloc_block_addr pc_a 1 in
+    let code := allocator_malloc_instrs_n 1 in
+    allocatorLayoutWf ->
+    ↑Nallocator ⊆ E ->
+    ContiguousRegion pc_a (length allocator_malloc_instrs) ->
+    SubBounds pc_b pc_e pc_a (pc_a ^+ length allocator_malloc_instrs)%a ->
+    disjoint_from_shadow pc_b pc_e ->
+    (0 < n)%Z ->
+    (n <= heap_e - next)%Z ->
+
+    allocator_ctx
+    ∗ allocator_service_data next
+    ∗ ▷ PC ↦ᵣ WCap true RX Global pc_b pc_e start
+    ∗ ▷ cgp ↦ᵣ WCap true RW Global
+        allocator_cgp_b allocator_cgp_e allocator_cgp_b
+    ∗ ▷ ca0 ↦ᵣ WInt n
+    ∗ ▷ ct0 ↦ᵣ w0
+    ∗ ▷ ct1 ↦ᵣ w1
+    ∗ ▷ ct2 ↦ᵣ w2
+    ∗ ▷ ct3 ↦ᵣ w3
+    ∗ ▷ ct4 ↦ᵣ w4
+    ∗ ▷ ca2 ↦ᵣ wa2
+    ∗ ▷ codefrag start code
+    ∗ ▷ (allocator_service_data next
+         ∗ cgp ↦ᵣ WCap true RW Global
+             allocator_cgp_b allocator_cgp_e allocator_cgp_b
+         ∗ ca0 ↦ᵣ WInt n
+         ∗ ct0 ↦ᵣ WCap true RW Global heap_b heap_e next
+         ∗ ct1 ↦ᵣ WInt next
+         ∗ codefrag start code
+         ∗ (∃ finish : Addr,
+             ⌜(next + n)%a = Some finish
+               ∧ (next < finish /\ finish <= heap_e)%a⌝
+             ∗ PC ↦ᵣ WCap true RX Global pc_b pc_e
+                 (allocator_malloc_block_addr pc_a 2)
+             ∗ ct2 ↦ᵣ WInt finish
+             ∗ ct3 ↦ᵣ WInt 0
+             ∗ ct4 ↦ᵣ WCap true RW Global next finish next
+             ∗ ca2 ↦ᵣ WCap true RW Global next finish next)
+         -∗ WP Seq (Instr Executable) @ E {{ φ }})
+    ⊢ WP Seq (Instr Executable) @ E {{ φ }}.
+  Proof.
+    intros start code Hlayout HE Hcont Hpc Hdisjoint Hpositive Hroom; subst start code.
+    iIntros "(#Hctx & Hdata & >HPC & >Hcgp & >Hca0 & >Hct0 & >Hct1 & >Hct2 & >Hct3 & >Hct4 & >Hca2 & >Hcode & Hφ)".
+    iDestruct "Hdata" as "(%Hnext & Hslot & Hroot & Hfree)".
+    codefrag_facts "Hcode".
+    assert (Hstart : allocator_malloc_block_addr pc_a 1 = (pc_a ^+ 6)%a) by reflexivity.
+    iEval (rewrite Hstart) in "Hcode".
+    iEval (rewrite Hstart) in "HPC".
+    rewrite Hstart in H.
+
+    (* Load ct0 cgp: the reserved root token proves the stored heap
+       capability's shadow bit is clear, so the load preserves its tag. *)
+    iInstr_lookup "Hcode" as "Hi" "Hcode".
+    wp_instr.
+    iDestruct (allocator_free_cell_shadow_access heap_b with "Hctx") as "#Haccess".
+    { apply elem_of_heap_addresses. apply withinBounds_true_iff.
+      pose proof heap_valid. solve_addr. }
+    iApply (wp_atomic _ _ (E ∖ ↑Nallocator)).
+    iMod ("Haccess" $! E HE with "Hroot") as (bit Hbit) "[Hs Hclose]".
+    subst bit. iModIntro.
+    iApply (wp_load_success_heap with "[$HPC $Hi $Hct0 $Hcgp $Hslot $Hs]"); try solve_pure.
+    { eapply (disjoint_from_shadow_not_in allocator_cgp_b allocator_cgp_e allocator_cgp_b).
+      { pose proof (@allocator_regions_disjoint MP layout Hlayout) as Hregions.
+        unfold disjoint_from_shadow. rewrite !disjoint_list_cons in Hregions.
+        cbn [union_list] in Hregions. set_solver. }
+      { apply withinBounds_true_iff.
+        pose proof (@allocator_size_data MP layout Hlayout) as Hsize.
+        cbn in Hsize. solve_addr. } }
+    { unfold is_heap_address. apply withinBounds_true_iff.
+      pose proof heap_valid. solve_addr. }
+    { split; first done. apply withinBounds_true_iff.
+      pose proof (@allocator_size_data MP layout Hlayout) as Hsize.
+      cbn in Hsize. solve_addr. }
+    iIntros "!> (HPC & Hct0 & Hi & Hcgp & Hslot & Hs)".
+    iMod ("Hclose" with "Hs") as "Hroot".
+    iModIntro. wp_pure.
+    iSpecialize ("Hcode" with "Hi").
+    codefrag_facts "Hcode".
+    assert (Hstep : (pc_a ^+ 7)%a = ((pc_a ^+ 6)%a ^+ 1)%a) by solve_addr.
+    iEval (rewrite Hstep) in "HPC".
+    iEval (simpl) in "Hct0".
+
+    (* GetA ct1 ct0. *)
+    iInstr "Hcode".
+    (* GetE ct2 ct0. *)
+    iInstr "Hcode".
+    (* Sub ct3 ct2 ct1 computes remaining capacity. *)
+    iInstr "Hcode".
+    (* Lt ct3 ct3 ca0 tests whether the request exceeds capacity. *)
+    iInstr "Hcode".
+    replace (heap_e - next <? n)%Z with false by (symmetry; apply Z.ltb_ge; lia).
+    (* Jnz .malloc_no_memory ct3 falls through. *)
+    iInstr "Hcode".
+    (* Add ct2 ct1 ca0 computes the end. *)
+    iInstr "Hcode".
+    (* Mov ct4 ct0 copies the heap capability. *)
+    iInstr "Hcode".
+    (* Subseg ct4 ct1 ct2 narrows it to the requested interval. *)
+    iInstr "Hcode".
+    (* Mov ca2 ct4 copies the bounded capability for zeroing. *)
+    iInstr "Hcode".
+    assert (Hfinish : (next + n)%a = Some (next ^+ n)%a) by solve_addr.
+    assert (Hnew : (next < (next ^+ n)%a /\ (next ^+ n)%a <= heap_e)%a) by solve_addr.
+    iApply "Hφ".
+    iSplitL "Hslot Hroot Hfree".
+    { iFrame. done. }
+    iFrame "Hcgp Hca0 Hct0 Hct1 Hcode".
+    iExists (next ^+ n)%a.
+    iSplit; first (iPureIntro; split; [exact Hfinish|exact Hnew]).
+    replace (allocator_malloc_block_addr pc_a 2) with (pc_a ^+ 16)%a by reflexivity.
+    assert (Hnextpc : ((pc_a ^+ 6)%a ^+ 10)%a = (pc_a ^+ 16)%a) by solve_addr.
+    iEval (rewrite Hnextpc) in "HPC".
+    replace (next ^+ (0 + n))%a with (next ^+ n)%a by solve_addr.
+    iFrame.
+    assert (Hword : WInt (next + n) = WInt (next ^+ n)%a) by (f_equal; solve_addr).
+    iEval (rewrite Hword) in "Hct2". iFrame.
+  Qed.
+
+  Lemma allocator_malloc_prepare_oom_spec
+    (E : coPset)
+    (pc_b pc_e pc_a next : Addr) (n : Z)
+    (w0 w1 w2 w3 w4 wa2 : Word)
+    (φ : language.val griotte_lang → iPropI Σ) :
+
+    let start := allocator_malloc_block_addr pc_a 1 in
+    let code := allocator_malloc_instrs_n 1 in
+    allocatorLayoutWf ->
+    ↑Nallocator ⊆ E ->
+    ContiguousRegion pc_a (length allocator_malloc_instrs) ->
+    SubBounds pc_b pc_e pc_a (pc_a ^+ length allocator_malloc_instrs)%a ->
+    disjoint_from_shadow pc_b pc_e ->
+    (0 < n)%Z ->
+    (heap_e - next < n)%Z ->
+
+    allocator_ctx
+    ∗ allocator_service_data next
+    ∗ ▷ PC ↦ᵣ WCap true RX Global pc_b pc_e start
+    ∗ ▷ cgp ↦ᵣ WCap true RW Global
+        allocator_cgp_b allocator_cgp_e allocator_cgp_b
+    ∗ ▷ ca0 ↦ᵣ WInt n
+    ∗ ▷ ct0 ↦ᵣ w0
+    ∗ ▷ ct1 ↦ᵣ w1
+    ∗ ▷ ct2 ↦ᵣ w2
+    ∗ ▷ ct3 ↦ᵣ w3
+    ∗ ▷ ct4 ↦ᵣ w4
+    ∗ ▷ ca2 ↦ᵣ wa2
+    ∗ ▷ codefrag start code
+    ∗ ▷ (allocator_service_data next
+         ∗ cgp ↦ᵣ WCap true RW Global
+             allocator_cgp_b allocator_cgp_e allocator_cgp_b
+         ∗ ca0 ↦ᵣ WInt n
+         ∗ ct0 ↦ᵣ WCap true RW Global heap_b heap_e next
+         ∗ ct1 ↦ᵣ WInt next
+         ∗ codefrag start code
+         ∗ PC ↦ᵣ WCap true RX Global pc_b pc_e
+             (allocator_malloc_block_addr pc_a 8)
+         ∗ ct2 ↦ᵣ WInt heap_e
+         ∗ ct3 ↦ᵣ WInt 1
+         ∗ ct4 ↦ᵣ w4
+         ∗ ca2 ↦ᵣ wa2
+         -∗ WP Seq (Instr Executable) @ E {{ φ }})
+    ⊢ WP Seq (Instr Executable) @ E {{ φ }}.
+  Proof.
+    intros start code Hlayout HE Hcont Hpc Hdisjoint Hpositive Hoom; subst start code.
+    iIntros "(#Hctx & Hdata & >HPC & >Hcgp & >Hca0 & >Hct0 & >Hct1 & >Hct2 & >Hct3 & >Hct4 & >Hca2 & >Hcode & Hφ)".
+    iDestruct "Hdata" as "(%Hnext & Hslot & Hroot & Hfree)".
+    codefrag_facts "Hcode".
+    assert (Hstart : allocator_malloc_block_addr pc_a 1 = (pc_a ^+ 6)%a) by reflexivity.
+    iEval (rewrite Hstart) in "Hcode".
+    iEval (rewrite Hstart) in "HPC".
+    rewrite Hstart in H.
+
+    (* Load ct0 cgp: the reserved root token proves the stored heap
+       capability's shadow bit is clear, so the load preserves its tag. *)
+    iInstr_lookup "Hcode" as "Hi" "Hcode".
+    wp_instr.
+    iDestruct (allocator_free_cell_shadow_access heap_b with "Hctx") as "#Haccess".
+    { apply elem_of_heap_addresses. apply withinBounds_true_iff.
+      pose proof heap_valid. solve_addr. }
+    iApply (wp_atomic _ _ (E ∖ ↑Nallocator)).
+    iMod ("Haccess" $! E HE with "Hroot") as (bit Hbit) "[Hs Hclose]".
+    subst bit. iModIntro.
+    iApply (wp_load_success_heap with "[$HPC $Hi $Hct0 $Hcgp $Hslot $Hs]"); try solve_pure.
+    { eapply (disjoint_from_shadow_not_in allocator_cgp_b allocator_cgp_e allocator_cgp_b).
+      { pose proof (@allocator_regions_disjoint MP layout Hlayout) as Hregions.
+        unfold disjoint_from_shadow. rewrite !disjoint_list_cons in Hregions.
+        cbn [union_list] in Hregions. set_solver. }
+      { apply withinBounds_true_iff.
+        pose proof (@allocator_size_data MP layout Hlayout) as Hsize.
+        cbn in Hsize. solve_addr. } }
+    { unfold is_heap_address. apply withinBounds_true_iff.
+      pose proof heap_valid. solve_addr. }
+    { split; first done. apply withinBounds_true_iff.
+      pose proof (@allocator_size_data MP layout Hlayout) as Hsize.
+      cbn in Hsize. solve_addr. }
+    iIntros "!> (HPC & Hct0 & Hi & Hcgp & Hslot & Hs)".
+    iMod ("Hclose" with "Hs") as "Hroot".
+    iModIntro. wp_pure.
+    iSpecialize ("Hcode" with "Hi").
+    codefrag_facts "Hcode".
+    assert (Hstep : (pc_a ^+ 7)%a = ((pc_a ^+ 6)%a ^+ 1)%a) by solve_addr.
+    iEval (rewrite Hstep) in "HPC".
+    iEval (simpl) in "Hct0".
+
+    (* GetA ct1 ct0. *)
+    iInstr "Hcode".
+    (* GetE ct2 ct0. *)
+    iInstr "Hcode".
+    (* Sub ct3 ct2 ct1 computes remaining capacity. *)
+    iInstr "Hcode".
+    (* Lt ct3 ct3 ca0 tests whether the request exceeds capacity. *)
+    iInstr "Hcode".
+    replace (heap_e - next <? n)%Z with true by (symmetry; apply Z.ltb_lt; lia).
+    (* Jnz to the out-of-memory block. *)
+    iInstr_lookup "Hcode" as "Hi" "Hcode".
+    wp_instr.
+    iApply (wp_jnz_success_jmp_z with "[$HPC $Hi $Hct3]"); try solve_pure.
+    { instantiate (1 := (pc_a ^+ 46)%a). solve_addr. }
+    iIntros "!> (HPC & Hi & Hct3)". wp_pure.
+    iSpecialize ("Hcode" with "Hi").
+    iApply "Hφ". iFrame.
+    done.
+  Qed.
+
+  Lemma allocator_malloc_publish_spec
+    (E : coPset)
+    (pc_b pc_e pc_a next finish : Addr) (n : Z) (wstatus : Word)
+    (φ : language.val griotte_lang → iPropI Σ) :
+
+    let start := allocator_malloc_block_addr pc_a 6 in
+    let code := allocator_malloc_instrs_n 6 in
+    allocatorLayoutWf ->
+    ContiguousRegion pc_a (length allocator_malloc_instrs) ->
+    SubBounds pc_b pc_e pc_a (pc_a ^+ length allocator_malloc_instrs)%a ->
+    disjoint_from_shadow pc_b pc_e ->
+    (next + n)%a = Some finish ->
+    (heap_b < next /\ next < finish /\ finish <= heap_e)%a ->
+
+    ▷ PC ↦ᵣ WCap true RX Global pc_b pc_e start
+    ∗ ▷ cgp ↦ᵣ WCap true RW Global
+        allocator_cgp_b allocator_cgp_e allocator_cgp_b
+    ∗ ▷ ct0 ↦ᵣ WCap true RW Global heap_b heap_e next
+    ∗ ▷ ct4 ↦ᵣ WCap true RW Global next finish next
+    ∗ ▷ ca0 ↦ᵣ WInt n
+    ∗ ▷ ca1 ↦ᵣ wstatus
+    ∗ ▷ allocator_cgp_b ↦ₐ WCap true RW Global heap_b heap_e next
+    ∗ ▷ codefrag start code
+    ∗ ▷ (PC ↦ᵣ WCap true RX Global pc_b pc_e
+           (allocator_malloc_block_addr pc_a 9)
+         ∗ cgp ↦ᵣ WCap true RW Global
+             allocator_cgp_b allocator_cgp_e allocator_cgp_b
+         ∗ ct0 ↦ᵣ WCap true RW Global heap_b heap_e finish
+         ∗ ct4 ↦ᵣ WCap true RW Global next finish next
+         ∗ ca0 ↦ᵣ WCap true RW Global next finish next
+         ∗ ca1 ↦ᵣ WInt ALLOC_OK
+         ∗ allocator_cgp_b ↦ₐ WCap true RW Global heap_b heap_e finish
+         ∗ codefrag start code
+         -∗ WP Seq (Instr Executable) @ E {{ φ }})
+    ⊢ WP Seq (Instr Executable) @ E {{ φ }}.
+  Proof.
+    intros start code Hlayout Hcont Hpc Hdisjoint Hfinish Hrange; subst start code.
+    iIntros "(>HPC & >Hcgp & >Hct0 & >Hct4 & >Hca0 & >Hca1 & >Hslot & >Hcode & Hφ)".
+    codefrag_facts "Hcode".
+    (* Lea ct0 ca0 computes the new bump cursor. *)
+    iInstr "Hcode".
+    assert (Hstart : allocator_malloc_block_addr pc_a 6 = (pc_a ^+ 38)%a) by reflexivity.
+    iEval (rewrite Hstart) in "Hcode".
+    rewrite Hstart in H.
+    assert (Hstep : (pc_a ^+ 39)%a = ((pc_a ^+ 38)%a ^+ 1)%a) by solve_addr.
+    iEval (rewrite Hstep) in "HPC".
+    (* Store cgp ct0 publishes the new cursor. *)
+    iInstr_lookup "Hcode" as "Hi" "Hcode".
+    wp_instr.
+    iApply (wp_store_success_reg _ _ _ _ _ _ _ _ _ _
+      (WCap true RW Global heap_b heap_e next)
+      with "[$HPC $Hi $Hct0 $Hcgp $Hslot]"); try solve_pure.
+    { eapply (disjoint_from_shadow_not_in allocator_cgp_b allocator_cgp_e allocator_cgp_b).
+      { pose proof (@allocator_regions_disjoint MP layout Hlayout) as Hregions.
+        unfold disjoint_from_shadow. rewrite !disjoint_list_cons in Hregions.
+        cbn [union_list] in Hregions. set_solver. }
+      { apply withinBounds_true_iff.
+        pose proof (@allocator_size_data MP layout Hlayout) as Hsize.
+        cbn in Hsize. solve_addr. } }
+    { rewrite <- Hstep. constructor; [solve_addr|done]. }
+    { apply withinBounds_true_iff.
+      pose proof (@allocator_size_data MP layout Hlayout) as Hsize.
+      cbn in Hsize. solve_addr. }
+    iIntros "!> (HPC & Hi & Hct0 & Hcgp & Hslot)". wp_pure.
+    iSpecialize ("Hcode" with "Hi").
+    (* Mov ca0 ct4. *)
+    iInstr "Hcode".
+    (* Mov ca1 ALLOC_OK. *)
+    iInstr "Hcode".
+    (* Jmp .malloc_return. *)
+    iInstr "Hcode".
+    iApply "Hφ". iFrame.
+    replace (allocator_malloc_block_addr pc_a 9) with (pc_a ^+ 48)%a by reflexivity.
+    assert (Hret : ((pc_a ^+ 38)%a ^+ 10)%a = (pc_a ^+ 48)%a) by solve_addr.
+    iEval (rewrite Hret) in "HPC". iFrame.
+  Qed.
+End AllocatorMallocBlocks.
+
+Section AllocatorMallocProof.
+  Context
+    {Σ : gFunctors}
+    {ceriseg : ceriseG Σ}
+    {allocatorg : allocatorG Σ}
+    {MP : MachineParameters}
+    {layout : allocatorLayout}
+    {layout_wf : allocatorLayoutWf}
+  .
+
+  (** A noninteger or nonpositive size is rejected before the heap is read.
+      Other registers and resources can be framed. *)
+  Lemma allocator_malloc_invalid_correct
+    (E : coPset) (wreq wret : Word)
+    (φ : language.val griotte_lang → iPropI Σ) :
+
+    ⊢ (⌜↑Nallocator ⊆ E⌝ -∗
+       ⌜↑Nallocator_service ⊆ E⌝ -∗
+       ⌜¬ allocator_positive_size wreq⌝ -∗
+
+       allocator_ctx ∗
+       allocator_service_ctx ∗
+       na_own cerise_nais E ∗
+
+       (* Initial register file. *)
+       PC ↦ᵣ WCap true RX Global allocator_pcc_b allocator_pcc_e
+         allocator_malloc_pcc_addr ∗
+       cgp ↦ᵣ WCap true RW Global
+         allocator_cgp_b allocator_cgp_e allocator_cgp_b ∗
+       cra ↦ᵣ wret ∗
+       ca0 ↦ᵣ wreq ∗
+       ca1 ↦ᵣ - ∗
+       ca2 ↦ᵣ - ∗
+       ct0 ↦ᵣ - ∗
+       ct1 ↦ᵣ - ∗
+       ct2 ↦ᵣ - ∗
+       ct3 ↦ᵣ - ∗
+       ct4 ↦ᵣ - ∗
+       ctp ↦ᵣ - ∗
+       cnull ↦ᵣ - ∗
+
+       ▷ (na_own cerise_nais E ∗
+          PC ↦ᵣ updatePcPerm wret ∗
+          cgp ↦ᵣ WCap true RW Global
+            allocator_cgp_b allocator_cgp_e allocator_cgp_b ∗
+          cra ↦ᵣ wret ∗
+          ca0 ↦ᵣ WInt 0 ∗
+          ca1 ↦ᵣ WInt ALLOC_INVALID ∗
+          ca2 ↦ᵣ - ∗
+          ct0 ↦ᵣ - ∗
+          ct1 ↦ᵣ - ∗
+          ct2 ↦ᵣ - ∗
+          ct3 ↦ᵣ - ∗
+          ct4 ↦ᵣ - ∗
+          ctp ↦ᵣ - ∗
+          cnull ↦ᵣ WInt 0
+
+          -∗ WP Seq (Instr Executable) @ E {{ φ }})
+       -∗ WP Seq (Instr Executable) @ E {{ φ }})%I.
+  Proof.
+    iIntros "%HEheap %HEservice %Hinvalid".
+    iIntros "(#Hctx & #Hservice & Hna & HPC & Hcgp & Hcra & Hca0 & Hca1 & Hca2 & Hct0 & Hct1 & Hct2 & Hct3 & Hct4 & Hctp & Hcnull & Hpost)".
+    (* Open the service invariant and recover the allocator code and state. *)
+    iMod (na_inv_acc with "Hservice Hna") as "(Hinv & Hna & Hclose)"; try exact HEservice.
+    iDestruct "Hinv" as ">[Hstatic Hdata]".
+    iDestruct "Hstatic" as "[Himports Hcode]".
+    iDestruct "Hdata" as (next) "Hdata".
+    iEval (rewrite /allocator_code) in "Hcode".
+    focus_block_0 "Hcode" as "Hmalloc_code" "Hcode_cont".
+    (* Check the requested size. *)
+    assert (Hsplit : allocator_malloc_instrs =
+      allocator_malloc_instrs_n 0 ++
+      concat (encodeInstrsW <$> drop 1 assembled_allocator_malloc)) by reflexivity.
+    iEval (rewrite Hsplit) in "Hmalloc_code".
+    focus_block_0 "Hmalloc_code" as "Hcheck_code" "Hmalloc_cont".
+    assert (Hpc : SubBounds allocator_pcc_b allocator_pcc_e
+      allocator_malloc_pcc_addr (allocator_malloc_pcc_addr ^+ length allocator_malloc_instrs)%a).
+    { pose proof allocator_size_code as Hsize_code.
+      pose proof allocator_size_imports as Himports_size.
+      rewrite /allocator_code length_app in Hsize_code.
+      unfold allocator_malloc_pcc_addr, allocator_malloc_pcc_off in *.
+      solve_addr. }
+    assert (Hdisjoint : disjoint_from_shadow allocator_pcc_b allocator_pcc_e).
+    { pose proof allocator_regions_disjoint as Hregions.
+      unfold disjoint_from_shadow.
+      rewrite !disjoint_list_cons in Hregions.
+      cbn [union_list] in Hregions.
+      set_solver. }
+    assert (Hstart : allocator_code_b = allocator_malloc_pcc_addr).
+    { pose proof allocator_size_imports as Hsize.
+      unfold allocator_malloc_pcc_addr, allocator_malloc_pcc_off in *.
+      solve_addr. }
+    iDestruct "Hct3" as (w3) "Hct3".
+    rewrite Hstart in H0.
+    iEval (rewrite Hstart) in "Hcheck_code".
+    iApply (allocator_malloc_size_check_invalid_spec with
+      "[- $HPC $Hca0 $Hct3 $Hcheck_code]"); eauto.
+    { rewrite -Hstart. exact H. }
+    iNext. iIntros "(Hca0 & Hct3 & Hcheck_code & HPC)".
+    iEval (rewrite -Hstart) in "Hcheck_code".
+    iDestruct ("Hmalloc_cont" with "Hcheck_code") as "Hmalloc_code".
+    iEval (rewrite -Hsplit) in "Hmalloc_code".
+    (* The size check rejects the request; set ALLOC_INVALID. *)
+    assert (Hsplit7 : allocator_malloc_instrs =
+      concat (encodeInstrsW <$> take 7 assembled_allocator_malloc) ++
+      (allocator_malloc_instrs_n 7 ++
+       concat (encodeInstrsW <$> drop 8 assembled_allocator_malloc)))
+      by reflexivity.
+    iEval (rewrite Hsplit7) in "Hmalloc_code".
+    focus_block_nochangePC 1 "Hmalloc_code" as a_reject Ha_reject
+      "Hreject_code" "Hmalloc_cont".
+    assert (Haddr7 : a_reject =
+      allocator_malloc_block_addr allocator_malloc_pcc_addr 7).
+    { rewrite -Hstart. unfold allocator_malloc_block_addr. solve_addr. }
+    subst a_reject.
+    iDestruct "Hca1" as (wca1) "Hca1".
+    iApply (allocator_malloc_reject_block_spec with
+      "[- $HPC $Hca0 $Hca1 $Hreject_code]"); eauto.
+    { rewrite -Hstart. exact H. }
+    iNext. iIntros "(HPC & Hca0 & Hca1 & Hreject_code)".
+    iDestruct ("Hmalloc_cont" with "Hreject_code") as "Hmalloc_code".
+    iEval (rewrite -Hsplit7) in "Hmalloc_code".
+    (* Return to the caller and restore the service invariant. *)
+    assert (Hsplit9 : allocator_malloc_instrs =
+      concat (encodeInstrsW <$> take 9 assembled_allocator_malloc) ++
+      allocator_malloc_instrs_n 9) by reflexivity.
+    iEval (rewrite Hsplit9) in "Hmalloc_code".
+    focus_block_nochangePC 1 "Hmalloc_code" as a_ret Ha_ret
+      "Hret_code" "Hmalloc_cont".
+    assert (Haddr9 : a_ret =
+      allocator_malloc_block_addr allocator_malloc_pcc_addr 9).
+    { rewrite -Hstart. unfold allocator_malloc_block_addr. solve_addr. }
+    subst a_ret.
+    assert (Hret_eq : allocator_malloc_instrs_n 9 =
+      encodeInstrsW [Jalr cnull cra]) by reflexivity.
+    iEval (rewrite Hret_eq) in "Hret_code".
+    iDestruct "Hcnull" as (wnull) "Hcnull".
+    iApply (allocator_return_spec with
+      "[- $HPC $Hcra $Hcnull $Hret_code]"); eauto.
+    { unfold allocator_malloc_block_addr in *. cbn. solve_addr. }
+    iNext. iIntros "(HPC & Hcra & Hcnull & Hret_code)".
+    iEval (rewrite -Hret_eq) in "Hret_code".
+    iDestruct ("Hmalloc_cont" with "Hret_code") as "Hmalloc_code".
+    iEval (rewrite -Hsplit9) in "Hmalloc_code".
+    iDestruct ("Hcode_cont" with "Hmalloc_code") as "Hcode".
+    iEval (rewrite -/allocator_code) in "Hcode".
+    iMod ("Hclose" with "[Himports Hcode Hdata Hna]") as "Hna".
+    { iSplitR "Hna"; last iFrame.
+      iNext. iSplitL "Himports Hcode"; first iFrame.
+      iExists next. iFrame. }
+    iApply "Hpost". iFrame "∗".
+  Qed.
+
+  (** A positive integer size either exceeds the remaining suffix or obtains
+      a fresh, exactly bounded, zeroed range. The bump cursor stays hidden in
+      the service invariant. *)
+  Lemma allocator_malloc_valid_correct
+    (E : coPset) (n : Z) (wret : Word)
+    (φ : language.val griotte_lang → iPropI Σ) :
+
+    ⊢ (⌜↑Nallocator ⊆ E⌝ -∗
+       ⌜↑Nallocator_service ⊆ E⌝ -∗
+       ⌜(0 < n)%Z⌝ -∗
+
+       allocator_ctx ∗
+       allocator_service_ctx ∗
+       na_own cerise_nais E ∗
+
+       (* Initial register file. *)
+       PC ↦ᵣ WCap true RX Global allocator_pcc_b allocator_pcc_e
+         allocator_malloc_pcc_addr ∗
+       cgp ↦ᵣ WCap true RW Global
+         allocator_cgp_b allocator_cgp_e allocator_cgp_b ∗
+       cra ↦ᵣ wret ∗
+       ca0 ↦ᵣ WInt n ∗
+       ca1 ↦ᵣ - ∗
+       ca2 ↦ᵣ - ∗
+       ct0 ↦ᵣ - ∗
+       ct1 ↦ᵣ - ∗
+       ct2 ↦ᵣ - ∗
+       ct3 ↦ᵣ - ∗
+       ct4 ↦ᵣ - ∗
+       ctp ↦ᵣ - ∗
+       cnull ↦ᵣ - ∗
+
+       ▷ (na_own cerise_nais E ∗
+          PC ↦ᵣ updatePcPerm wret ∗
+          cgp ↦ᵣ WCap true RW Global
+            allocator_cgp_b allocator_cgp_e allocator_cgp_b ∗
+          cra ↦ᵣ wret ∗
+          ca2 ↦ᵣ - ∗
+          ct0 ↦ᵣ - ∗
+          ct1 ↦ᵣ - ∗
+          ct2 ↦ᵣ - ∗
+          ct3 ↦ᵣ - ∗
+          ct4 ↦ᵣ - ∗
+          ctp ↦ᵣ - ∗
+          cnull ↦ᵣ WInt 0 ∗
+
+          ((ca0 ↦ᵣ WInt 0 ∗
+            ca1 ↦ᵣ WInt ALLOC_NO_MEMORY)
+           ∨ (∃ (b e : Addr),
+                ⌜(heap_b < b /\ b < e /\ e <= heap_e)%a ∧
+                  (e - b = n)%Z⌝ ∗
+                ca0 ↦ᵣ WCap true RW Global b e b ∗
+                ca1 ↦ᵣ WInt ALLOC_OK ∗
+                allocator_zeroed b e))
+
+          -∗ WP Seq (Instr Executable) @ E {{ φ }})
+       -∗ WP Seq (Instr Executable) @ E {{ φ }})%I.
+  Proof.
+    iIntros "%HEheap %HEservice %Hpositive".
+    iIntros "(#Hctx & #Hservice & Hna & HPC & Hcgp & Hcra & Hca0 & Hca1 & Hca2 & Hct0 & Hct1 & Hct2 & Hct3 & Hct4 & Hctp & Hcnull & Hpost)".
+    (* Open the service invariant and recover the allocator code and state. *)
+    iMod (na_inv_acc with "Hservice Hna") as "(Hinv & Hna & Hclose)"; try exact HEservice.
+    iDestruct "Hinv" as ">[Hstatic Hdata]".
+    iDestruct "Hstatic" as "[Himports Hcode]".
+    iDestruct "Hdata" as (next) "Hdata".
+    iEval (rewrite /allocator_code) in "Hcode".
+    focus_block_0 "Hcode" as "Hmalloc_code" "Hcode_cont".
+    (* Check the requested size. *)
+    assert (Hsplit : allocator_malloc_instrs =
+      allocator_malloc_instrs_n 0 ++
+      concat (encodeInstrsW <$> drop 1 assembled_allocator_malloc)) by reflexivity.
+    iEval (rewrite Hsplit) in "Hmalloc_code".
+    focus_block_0 "Hmalloc_code" as "Hcheck_code" "Hmalloc_cont".
+    assert (Hpc : SubBounds allocator_pcc_b allocator_pcc_e
+      allocator_malloc_pcc_addr
+      (allocator_malloc_pcc_addr ^+ length allocator_malloc_instrs)%a).
+    { pose proof allocator_size_code as Hsize_code.
+      pose proof allocator_size_imports as Himports_size.
+      rewrite /allocator_code length_app in Hsize_code.
+      unfold allocator_malloc_pcc_addr, allocator_malloc_pcc_off in *.
+      solve_addr. }
+    assert (Hdisjoint : disjoint_from_shadow allocator_pcc_b allocator_pcc_e).
+    { pose proof allocator_regions_disjoint as Hregions.
+      unfold disjoint_from_shadow.
+      rewrite !disjoint_list_cons in Hregions.
+      cbn [union_list] in Hregions.
+      set_solver. }
+    assert (Hstart : allocator_code_b = allocator_malloc_pcc_addr).
+    { pose proof allocator_size_imports as Hsize.
+      unfold allocator_malloc_pcc_addr, allocator_malloc_pcc_off in *.
+      solve_addr. }
+    iDestruct "Hct3" as (w3) "Hct3".
+    rewrite Hstart in H0.
+    iEval (rewrite Hstart) in "Hcheck_code".
+    assert (Hsize : allocator_positive_size (WInt n)).
+    { exists n. split; [reflexivity|exact Hpositive]. }
+    iApply (allocator_malloc_size_check_valid_spec with
+      "[- $HPC $Hca0 $Hct3 $Hcheck_code]"); eauto.
+    { rewrite -Hstart. exact H. }
+    iNext. iIntros "(Hca0 & Hct3 & Hcheck_code & HPC)".
+    iEval (rewrite -Hstart) in "Hcheck_code".
+    iDestruct ("Hmalloc_cont" with "Hcheck_code") as "Hmalloc_code".
+    iEval (rewrite -Hsplit) in "Hmalloc_code".
+    (* Prepare the allocation, branching on the remaining capacity. *)
+    assert (Hsplit1 : allocator_malloc_instrs =
+      concat (encodeInstrsW <$> take 1 assembled_allocator_malloc) ++
+      (allocator_malloc_instrs_n 1 ++
+       concat (encodeInstrsW <$> drop 2 assembled_allocator_malloc)))
+      by reflexivity.
+    iEval (rewrite Hsplit1) in "Hmalloc_code".
+    focus_block_nochangePC 1 "Hmalloc_code" as a_prepare Ha_prepare
+      "Hprepare_code" "Hmalloc_cont".
+    assert (Haddr1 : a_prepare =
+      allocator_malloc_block_addr allocator_malloc_pcc_addr 1).
+    { rewrite -Hstart. unfold allocator_malloc_block_addr. solve_addr. }
+    subst a_prepare.
+    iDestruct "Hct0" as (w0) "Hct0".
+    iDestruct "Hct1" as (w1) "Hct1".
+    iDestruct "Hct2" as (w2) "Hct2".
+    iDestruct "Hct3" as (w3b) "Hct3".
+    iDestruct "Hct4" as (w4) "Hct4".
+    iDestruct "Hca2" as (wa2) "Hca2".
+    destruct (decide (n <= heap_e - next)%Z) as [Hroom|Hoom].
+    - iApply (allocator_malloc_prepare_success_spec with
+        "[- $Hctx $Hdata $HPC $Hcgp $Hca0 $Hct0 $Hct1 $Hct2 $Hct3 $Hct4 $Hca2 $Hprepare_code]"); eauto.
+      { rewrite -Hstart. exact H. }
+      iNext. iIntros
+        "(Hdata & Hcgp & Hca0 & Hct0 & Hct1 & Hprepare_code & Hroom)".
+      iDestruct "Hroom" as (finish)
+        "(%Hfinish & HPC & Hct2 & Hct3 & Hct4 & Hca2)".
+      destruct Hfinish as [Hfinish Hrange].
+      iDestruct ("Hmalloc_cont" with "Hprepare_code") as "Hmalloc_code".
+      iEval (rewrite -Hsplit1) in "Hmalloc_code".
+      iDestruct "Hdata" as "(%Hnext & Hslot & Hroot & Hfree)".
+      (* Take ownership of the requested range from the free suffix. *)
+      assert (Hsplit_range : (next <= finish /\ finish <= heap_e)%a)
+        by solve_addr.
+      iEval (rewrite /free_cells
+        (finz_seq_between_split next finish heap_e Hsplit_range)
+        big_sepL_app) in "Hfree".
+      iDestruct "Hfree" as "[Hrange_free Hfree]".
+      iPoseProof (allocator_take_range_correct E next finish) as "Htake".
+      iSpecialize ("Htake" with
+        "[] [] Hctx Hrange_free").
+      { iPureIntro. exact HEheap. }
+      { iPureIntro. solve_addr. }
+      iMod "Htake" as "Hrange_mem".
+      (* Zero the newly allocated cells. *)
+      assert (Hsplit2 : allocator_malloc_instrs =
+        concat (encodeInstrsW <$> take 2 assembled_allocator_malloc) ++
+        (allocator_malloc_instrs_n 2 ++
+         concat (encodeInstrsW <$> drop 3 assembled_allocator_malloc)))
+        by reflexivity.
+      iEval (rewrite Hsplit2) in "Hmalloc_code".
+      focus_block_nochangePC 1 "Hmalloc_code" as a_zero Ha_zero
+        "Hzero_code" "Hmalloc_cont".
+      assert (Haddr2 : a_zero =
+        allocator_malloc_block_addr allocator_malloc_pcc_addr 2).
+      { rewrite -Hstart. unfold allocator_malloc_block_addr.
+        clear -Ha_zero. cbn [take concat fmap] in *. solve_addr. }
+      subst a_zero.
+      assert (Hzero_eq : allocator_malloc_instrs_n 2 =
+        allocator_zero_instrs ca2 ct2 ct3) by reflexivity.
+      iEval (rewrite Hzero_eq) in "Hzero_code".
+      iApply (allocator_zero_spec ca2 ct2 ct3 E RX Global
+        allocator_pcc_b allocator_pcc_e
+        (allocator_malloc_block_addr allocator_malloc_pcc_addr 2)
+        RW Global next finish (WInt 0)
+        with "[- $HPC $Hca2 $Hct2 $Hct3 $Hzero_code $Hrange_mem]").
+      { reflexivity. }
+      { unfold allocator_malloc_block_addr; cbn; solve_addr. }
+      { exact Hdisjoint. }
+      { reflexivity. }
+      { solve_addr. }
+      { vm_compute;
+        repeat (constructor;
+          [rewrite !elem_of_cons elem_of_nil; intuition congruence|]);
+        constructor.
+        { apply not_elem_of_nil. }
+        { constructor. } }
+      iNext. iIntros "(HPC & Hca2 & Hct2 & Hct3 & Hzero_code & Hzeros)".
+      iEval (rewrite -Hzero_eq) in "Hzero_code".
+      iDestruct ("Hmalloc_cont" with "Hzero_code") as "Hmalloc_code".
+      iEval (rewrite -Hsplit2) in "Hmalloc_code".
+      (* Fetch the shadow capability and translate the allocated bounds. *)
+      assert (Hsplit3 : allocator_malloc_instrs =
+        concat (encodeInstrsW <$> take 3 assembled_allocator_malloc) ++
+        (allocator_malloc_instrs_n 3 ++
+         concat (encodeInstrsW <$> drop 4 assembled_allocator_malloc)))
+        by reflexivity.
+      iEval (rewrite Hsplit3) in "Hmalloc_code".
+      focus_block_nochangePC 1 "Hmalloc_code" as a_fetch Ha_fetch
+        "Hfetch_code" "Hmalloc_cont".
+      assert (Haddr3 : a_fetch =
+        allocator_malloc_block_addr allocator_malloc_pcc_addr 3).
+      { rewrite -Hstart. unfold allocator_malloc_block_addr.
+        clear -Ha_fetch. cbn [take concat fmap] in *. solve_addr. }
+      subst a_fetch.
+      assert (Hpc3 : (allocator_malloc_block_addr allocator_malloc_pcc_addr 2 ^+
+        length (allocator_zero_instrs ca2 ct2 ct3))%a =
+        allocator_malloc_block_addr allocator_malloc_pcc_addr 3).
+      { unfold allocator_malloc_block_addr. clear -Hpc. solve_addr. }
+      iEval (rewrite Hpc3) in "HPC".
+      pose proof allocator_size_imports as Himports_size.
+      iDestruct (region_pointsto_single with "Himports") as (v)
+        "[Himport %Hentry]"; first exact Himports_size.
+      cbn in Hentry. inversion Hentry; subst v.
+      assert (Hfetch_eq : allocator_malloc_instrs_n 3 =
+        fetch.fetch_instrs allocator_shadow_import_off ctp ct3 ca2)
+        by reflexivity.
+      iEval (rewrite Hfetch_eq) in "Hfetch_code".
+      iDestruct "Hctp" as (wctp) "Hctp".
+      assert (Himpaddr : (allocator_pcc_b ^+ allocator_shadow_import_off)%a =
+        allocator_pcc_b)
+        by (unfold allocator_shadow_import_off; solve_addr).
+      iEval (rewrite -Himpaddr) in "Himport".
+      iApply (allocator_fetch_spec with
+        "[- $HPC $Hctp $Hct3 $Hca2 $Hfetch_code $Himport]").
+      { reflexivity. }
+      { rewrite -Hfetch_eq;
+        unfold allocator_malloc_block_addr; cbn; solve_addr. }
+      { apply withinBounds_true_iff; solve_addr. }
+      { exact Hdisjoint. }
+      { cbn [is_heap_cap]; unfold is_heap_address;
+        apply not_true_is_false; intro Hheap;
+        apply withinBounds_true_iff in Hheap;
+        pose proof heap_shadow_disjoint as Hd;
+        rewrite /disjoint_from_shadow elem_of_disjoint in Hd;
+        apply (Hd shadow_b); apply elem_of_finz_seq_between;
+        try exact Hheap;
+        pose proof shadow_valid; solve_addr. }
+      { discriminate. }
+      { discriminate. }
+      { discriminate. }
+      iNext. iIntros "(HPC & Hctp & Hct3 & Hca2 & Hfetch_code & Himport)".
+      iEval (cbn) in "Hctp".
+      iEval (rewrite Himpaddr) in "Himport".
+      iAssert ([[allocator_pcc_b,allocator_code_b]] ↦ₐ [[allocator_imports]])%I
+        with "[Himport]" as "Himports".
+      { rewrite /allocator_imports /region_pointsto
+          (finz_seq_between_singleton allocator_pcc_b allocator_code_b Himports_size) /=.
+        iFrame. }
+      iEval (rewrite -Hfetch_eq) in "Hfetch_code".
+      iDestruct ("Hmalloc_cont" with "Hfetch_code") as "Hmalloc_code".
+      iEval (rewrite -Hsplit3) in "Hmalloc_code".
+      assert (Hsplit4 : allocator_malloc_instrs =
+        concat (encodeInstrsW <$> take 4 assembled_allocator_malloc) ++
+        (allocator_malloc_instrs_n 4 ++
+         concat (encodeInstrsW <$> drop 5 assembled_allocator_malloc)))
+        by reflexivity.
+      iEval (rewrite Hsplit4) in "Hmalloc_code".
+      focus_block_nochangePC 1 "Hmalloc_code" as a_translate Ha_translate
+        "Htranslate_code" "Hmalloc_cont".
+      assert (Haddr4 : a_translate =
+        allocator_malloc_block_addr allocator_malloc_pcc_addr 4).
+      { rewrite -Hstart. unfold allocator_malloc_block_addr.
+        clear -Ha_translate. cbn [take concat fmap] in *. solve_addr. }
+      subst a_translate.
+      assert (Hpc4 : (allocator_malloc_block_addr allocator_malloc_pcc_addr 3 ^+
+        length (fetch.fetch_instrs allocator_shadow_import_off ctp ct3 ca2))%a =
+        allocator_malloc_block_addr allocator_malloc_pcc_addr 4).
+      { unfold allocator_malloc_block_addr. solve_addr. }
+      iEval (rewrite Hpc4) in "HPC".
+      iApply (allocator_translate_spec with
+        "[- $HPC $Hct0 $Hct1 $Hct2 $Hct3 $Hctp $Hca2 $Htranslate_code]");
+        eauto; try solve_addr.
+      iNext. iIntros
+        "(HPC & Hct0 & Hct1 & Hct2 & Hct3 & Hctp & Hca2 & Htranslate_code)".
+      iDestruct ("Hmalloc_cont" with "Htranslate_code") as "Hmalloc_code".
+      iEval (rewrite -Hsplit4) in "Hmalloc_code".
+      iAssert ([[next, finish]] ↦ₐ
+        [[replicate (length (finz.seq_between next finish)) (WInt 0)]])%I
+        with "[Hzeros]" as "Hzeros".
+      { rewrite /region_pointsto big_sepL2_replicate_r; last reflexivity.
+        iFrame. }
+      (* Clear the shadow bits for the allocated range. *)
+      assert (Hsplit5 : allocator_malloc_instrs =
+        concat (encodeInstrsW <$> take 5 assembled_allocator_malloc) ++
+        (allocator_malloc_instrs_n 5 ++
+         concat (encodeInstrsW <$> drop 6 assembled_allocator_malloc)))
+        by reflexivity.
+      iEval (rewrite Hsplit5) in "Hmalloc_code".
+      focus_block_nochangePC 1 "Hmalloc_code" as a_paint Ha_paint
+        "Hpaint_code" "Hmalloc_cont".
+      assert (Haddr5 : a_paint =
+        allocator_malloc_block_addr allocator_malloc_pcc_addr 5).
+      { rewrite -Hstart. unfold allocator_malloc_block_addr.
+        clear -Ha_paint. cbn [take concat fmap] in *. solve_addr. }
+      subst a_paint.
+      assert (Hpc5 : (allocator_malloc_block_addr allocator_malloc_pcc_addr 4 ^+
+        length (allocator_malloc_instrs_n 4))%a =
+        allocator_malloc_block_addr allocator_malloc_pcc_addr 5).
+      { unfold allocator_malloc_block_addr. solve_addr. }
+      iEval (rewrite Hpc5) in "HPC".
+      pose (sb := (shadow_b ^+ (next - heap_b))%a).
+      pose (se := (shadow_b ^+ (finish - heap_b))%a).
+      assert (Hshadow : (shadow_b <= sb /\ sb < se /\ se <= shadow_e)%a).
+      { pose proof heap_shadow_same_size. unfold sb, se. solve_addr. }
+      assert (Hlen_shadow : (se - sb = finish - next)%Z).
+      { unfold sb, se. pose proof heap_shadow_same_size. solve_addr. }
+      assert (Htranslation : ∀ x, (next <= x /\ x < finish)%a ->
+        heap_to_shadow x = Some (sb ^+ (x - next))%a).
+      { intros x Hx. rewrite allocator_translation_affine.
+        unfold translate_region.
+        assert (Hxheap : withinBounds heap_b heap_e x = true).
+        { apply withinBounds_true_iff. solve_addr. }
+        rewrite Hxheap. unfold sb.
+        pose proof heap_shadow_same_size. solve_addr. }
+      assert (Hpaint_eq : allocator_malloc_instrs_n 5 =
+        allocator_paint_instrs ctp ca2 false) by reflexivity.
+      iEval (rewrite Hpaint_eq) in "Hpaint_code".
+      iApply (allocator_paint_spec false ctp ca2 E RX Global
+        allocator_pcc_b allocator_pcc_e
+        (allocator_malloc_block_addr allocator_malloc_pcc_addr 5)
+        next finish sb se
+        (replicate (length (finz.seq_between next finish)) (WInt 0))
+        with "[- $Hctx $HPC $Hctp $Hca2 $Hpaint_code $Hzeros]").
+      { reflexivity. }
+      { rewrite -Hpaint_eq;
+        unfold allocator_malloc_block_addr; cbn; solve_addr. }
+      { exact Hdisjoint. }
+      { exact HEheap. }
+      { solve_addr. }
+      { exact Hshadow. }
+      { exact Hlen_shadow. }
+      { exact Htranslation. }
+      { vm_compute;
+        repeat (constructor;
+          [rewrite !elem_of_cons elem_of_nil; intuition congruence|]);
+        try apply not_elem_of_nil; constructor.
+        { apply not_elem_of_nil. }
+        { constructor. } }
+      iNext. iIntros "(HPC & Hctp & Hca2 & Hpaint_code & Hzeros)".
+      iEval (rewrite -Hpaint_eq) in "Hpaint_code".
+      iDestruct ("Hmalloc_cont" with "Hpaint_code") as "Hmalloc_code".
+      iEval (rewrite -Hsplit5) in "Hmalloc_code".
+      (* Publish the new bump cursor and set ALLOC_OK. *)
+      assert (Hsplit6 : allocator_malloc_instrs =
+        concat (encodeInstrsW <$> take 6 assembled_allocator_malloc) ++
+        (allocator_malloc_instrs_n 6 ++
+         concat (encodeInstrsW <$> drop 7 assembled_allocator_malloc)))
+        by reflexivity.
+      iEval (rewrite Hsplit6) in "Hmalloc_code".
+      focus_block_nochangePC 1 "Hmalloc_code" as a_publish Ha_publish
+        "Hpublish_code" "Hmalloc_cont".
+      assert (Haddr6 : a_publish =
+        allocator_malloc_block_addr allocator_malloc_pcc_addr 6).
+      { rewrite -Hstart. unfold allocator_malloc_block_addr.
+        clear -Ha_publish. cbn [take concat fmap] in *. solve_addr. }
+      subst a_publish.
+      assert (Hoff5 : allocator_malloc_block_addr allocator_malloc_pcc_addr 5 =
+        (allocator_malloc_pcc_addr ^+ 34)%a) by reflexivity.
+      assert (Hoff6 : allocator_malloc_block_addr allocator_malloc_pcc_addr 6 =
+        (allocator_malloc_pcc_addr ^+ 38)%a) by reflexivity.
+      assert (Hlenpaint : length (allocator_paint_instrs ctp ca2 false) = 4)
+        by reflexivity.
+      assert (Hpc6 : (allocator_malloc_block_addr allocator_malloc_pcc_addr 5 ^+
+        length (allocator_paint_instrs ctp ca2 false))%a =
+        allocator_malloc_block_addr allocator_malloc_pcc_addr 6).
+      { clear -Hoff5 Hoff6 Hlenpaint.
+        rewrite Hoff5 Hoff6 Hlenpaint.
+        rewrite incr_addr_opt_add_twice.
+        { replace (34 + 4)%Z with 38%Z by lia; reflexivity. }
+        all: lia. }
+      iEval (rewrite Hpc6) in "HPC".
+      iDestruct "Hca1" as (wca1) "Hca1".
+      iApply (allocator_malloc_publish_spec with
+        "[- $HPC $Hcgp $Hct0 $Hct4 $Hca0 $Hca1 $Hslot $Hpublish_code]").
+      { rewrite -Hstart; exact H. }
+      { exact Hpc. }
+      { exact Hdisjoint. }
+      { exact Hfinish. }
+      { split; [exact (proj1 Hnext)|exact Hrange]. }
+      iNext. iIntros
+        "(HPC & Hcgp & Hct0 & Hct4 & Hca0 & Hca1 & Hslot & Hpublish_code)".
+      iDestruct ("Hmalloc_cont" with "Hpublish_code") as "Hmalloc_code".
+      iEval (rewrite -Hsplit6) in "Hmalloc_code".
+      (* Return the allocation and restore the service invariant. *)
+      assert (Hsplit9 : allocator_malloc_instrs =
+        concat (encodeInstrsW <$> take 9 assembled_allocator_malloc) ++
+        allocator_malloc_instrs_n 9) by reflexivity.
+      iEval (rewrite Hsplit9) in "Hmalloc_code".
+      focus_block_nochangePC 1 "Hmalloc_code" as a_ret Ha_ret
+        "Hret_code" "Hmalloc_cont".
+      assert (Haddr9 : a_ret =
+        allocator_malloc_block_addr allocator_malloc_pcc_addr 9).
+      { rewrite -Hstart. unfold allocator_malloc_block_addr.
+        clear -Ha_ret. cbn [take concat fmap] in *. solve_addr. }
+      subst a_ret.
+      assert (Hret_eq : allocator_malloc_instrs_n 9 =
+        encodeInstrsW [Jalr cnull cra]) by reflexivity.
+      iEval (rewrite Hret_eq) in "Hret_code".
+      iDestruct "Hcnull" as (wnull) "Hcnull".
+      iApply (allocator_return_spec with
+        "[- $HPC $Hcra $Hcnull $Hret_code]").
+      { unfold allocator_malloc_block_addr in *; cbn; solve_addr. }
+      { exact Hdisjoint. }
+      iNext. iIntros "(HPC & Hcra & Hcnull & Hret_code)".
+      iEval (rewrite -Hret_eq) in "Hret_code".
+      iDestruct ("Hmalloc_cont" with "Hret_code") as "Hmalloc_code".
+      iEval (rewrite -Hsplit9) in "Hmalloc_code".
+      iDestruct ("Hcode_cont" with "Hmalloc_code") as "Hcode".
+      iEval (rewrite -/allocator_code) in "Hcode".
+      iMod ("Hclose" with "[Himports Hcode Hslot Hroot Hfree Hna]") as "Hna".
+      { iSplitR "Hna"; last iFrame.
+        iNext. iSplitL "Himports Hcode"; first iFrame.
+        iExists finish. iFrame. iPureIntro.
+        clear -Hnext Hrange. solve_addr. }
+      iApply "Hpost". iFrame "∗".
+      iRight. iExists next, finish.
+      iSplit.
+      { iPureIntro. split.
+        { split; [exact (proj1 Hnext)|exact Hrange]. }
+        { clear -Hfinish. solve_addr. } }
+      iFrame.
+      rewrite /allocator_zeroed /region_pointsto big_sepL2_replicate_r;
+        last reflexivity.
+      iFrame.
+    - assert (Hcapacity : (heap_e - next < n)%Z) by lia.
+      iApply (allocator_malloc_prepare_oom_spec with
+        "[- $Hctx $Hdata $HPC $Hcgp $Hca0 $Hct0 $Hct1 $Hct2 $Hct3 $Hct4 $Hca2 $Hprepare_code]"); eauto.
+      { rewrite -Hstart. exact H. }
+      iNext. iIntros
+        "(Hdata & Hcgp & Hca0 & Hct0 & Hct1 & Hprepare_code & HPC & Hct2 & Hct3 & Hct4 & Hca2)".
+      iDestruct ("Hmalloc_cont" with "Hprepare_code") as "Hmalloc_code".
+      iEval (rewrite -Hsplit1) in "Hmalloc_code".
+      (* Capacity is exhausted; return ALLOC_NO_MEMORY without changing the state. *)
+      assert (Hsplit8 : allocator_malloc_instrs =
+        concat (encodeInstrsW <$> take 8 assembled_allocator_malloc) ++
+        (allocator_malloc_instrs_n 8 ++ allocator_malloc_instrs_n 9))
+        by reflexivity.
+      iEval (rewrite Hsplit8) in "Hmalloc_code".
+      focus_block_nochangePC 1 "Hmalloc_code" as a_oom Ha_oom
+        "Hoom_code" "Hmalloc_cont".
+      assert (Haddr8 : a_oom =
+        allocator_malloc_block_addr allocator_malloc_pcc_addr 8).
+      { rewrite -Hstart. unfold allocator_malloc_block_addr.
+        clear -Ha_oom. cbn [take concat fmap] in *. solve_addr. }
+      subst a_oom.
+      iDestruct "Hca1" as (wca1) "Hca1".
+      iApply (allocator_malloc_oom_block_spec with
+        "[- $HPC $Hca0 $Hca1 $Hoom_code]").
+      { rewrite -Hstart; exact H. }
+      { exact Hpc. }
+      { exact Hdisjoint. }
+      iNext. iIntros "(HPC & Hca0 & Hca1 & Hoom_code)".
+      iDestruct ("Hmalloc_cont" with "Hoom_code") as "Hmalloc_code".
+      iEval (rewrite -Hsplit8) in "Hmalloc_code".
+      assert (Hsplit9 : allocator_malloc_instrs =
+        concat (encodeInstrsW <$> take 9 assembled_allocator_malloc) ++
+        allocator_malloc_instrs_n 9) by reflexivity.
+      iEval (rewrite Hsplit9) in "Hmalloc_code".
+      focus_block_nochangePC 1 "Hmalloc_code" as a_ret Ha_ret
+        "Hret_code" "Hmalloc_cont".
+      assert (Haddr9 : a_ret =
+        allocator_malloc_block_addr allocator_malloc_pcc_addr 9).
+      { rewrite -Hstart. unfold allocator_malloc_block_addr.
+        clear -Ha_ret. cbn [take concat fmap] in *. solve_addr. }
+      subst a_ret.
+      assert (Hret_eq : allocator_malloc_instrs_n 9 =
+        encodeInstrsW [Jalr cnull cra]) by reflexivity.
+      iEval (rewrite Hret_eq) in "Hret_code".
+      iDestruct "Hcnull" as (wnull) "Hcnull".
+      iApply (allocator_return_spec with
+        "[- $HPC $Hcra $Hcnull $Hret_code]").
+      { unfold allocator_malloc_block_addr in *; cbn; solve_addr. }
+      { exact Hdisjoint. }
+      iNext. iIntros "(HPC & Hcra & Hcnull & Hret_code)".
+      iEval (rewrite -Hret_eq) in "Hret_code".
+      iDestruct ("Hmalloc_cont" with "Hret_code") as "Hmalloc_code".
+      iEval (rewrite -Hsplit9) in "Hmalloc_code".
+      iDestruct ("Hcode_cont" with "Hmalloc_code") as "Hcode".
+      iEval (rewrite -/allocator_code) in "Hcode".
+      iMod ("Hclose" with "[Himports Hcode Hdata Hna]") as "Hna".
+      { iSplitR "Hna"; last iFrame.
+        iNext. iSplitL "Himports Hcode"; first iFrame.
+        iExists next. iFrame. }
+      iApply "Hpost". iFrame "∗". iLeft. iFrame.
+  Qed.
+End AllocatorMallocProof.
